Event_Safe.thy
@@ -158,215 +158,6 @@ theorem erule_frame:
   \<Longrightarrow> \<Gamma> \<turnstile>\<^sub>e {P ** R} e {Q ** R}"
   by (auto simp add: eCSL_def intro: esafe_frame)
 
-subsection \<open>specification and proof rules for resource events\<close>
-
-primrec 
-  resafe :: "nat \<Rightarrow> revent \<Rightarrow> stack \<Rightarrow> heap \<Rightarrow> (rname \<Rightarrow> assn) \<Rightarrow> assn \<Rightarrow> bool"
-where
-  "resafe 0 e s h \<Gamma> Q = True"
-| "resafe (Suc n) re s h \<Gamma> Q = (
-  (snd re = AnonyEvent Cskip \<longrightarrow> (s, h) \<Turnstile> Q)
-\<and> (\<forall>hF. disjoint (dom h) (dom hF) \<longrightarrow> \<not> reaborts re (s, h ++ hF))
-\<and> (reaccesses re s \<subseteq> dom h)
-\<and> (\<forall>hJ hF re' \<sigma>' x x' actk. 
-      (re, (s, h ++ hJ ++ hF), x) -ret-actk\<rightarrow> (re', \<sigma>', x')
-    \<longrightarrow> (s, hJ) \<Turnstile> envs \<Gamma> (rellocked re') (rellocked re)
-    \<longrightarrow> (disjoint (dom h) (dom hJ) \<and> disjoint (dom h) (dom hF) \<and> disjoint (dom hJ) (dom hF))
-    \<longrightarrow> (\<exists>h' hJ'.
-            snd \<sigma>' = h' ++ hJ' ++ hF
-          \<and> disjoint (dom h') (dom hJ') \<and> disjoint (dom h') (dom hF) \<and> disjoint (dom hJ') (dom hF)
-          \<and> (fst \<sigma>', hJ') \<Turnstile> envs \<Gamma> (rellocked re) (rellocked re')
-          \<and> resafe n re' (fst \<sigma>') h' \<Gamma> Q)))"
-
-lemma resafe_mon:
-  "\<lbrakk> resafe n re s h \<Gamma> Q; m \<le> n \<rbrakk> \<Longrightarrow> resafe m re s h \<Gamma> Q"
-apply (induct m arbitrary: re s n h, simp) 
-apply (case_tac n, clarify)
-apply (simp only: safe.simps, clarsimp)
-  apply (drule_tac a = hJ and b = hF and c = aa and d = ba and e = ab and f = bb in all6D, drule imp3D, simp_all)
-   apply blast
-  apply (clarsimp, rule_tac x="h'" in exI, rule_tac x="hJ'" in exI, simp)
-  done 
-
-lemma resafe_agrees: 
-    "\<lbrakk> resafe n re s h \<Gamma> Q ; 
-     agrees (fvREv re \<union> fvA Q \<union> fvAs \<Gamma>) s s' \<rbrakk>
-   \<Longrightarrow> resafe n re s' h \<Gamma> Q"
-  apply (induct n arbitrary: re s s' h, simp, simp only: resafe.simps, clarify)
-  apply (rule conjI, clarsimp, subst assn_agrees, subst agreesC, assumption+)
-  apply (rule conjI, clarsimp)
-   apply (drule_tac reaborts_agrees, simp, fast, simp, simp)
-  apply (rule conjI, subst (asm) reaccesses_agrees, simp_all)
-  apply (clarify, drule_tac X = "fvREv (a, b) \<union> fvAs \<Gamma> \<union> fvA Q" in rered_agrees,
-       simp (no_asm), fast, simp(no_asm), fast, clarify)
-  apply (drule_tac a = hJ and b = hF and c = aa and d = ba and e = s'a and f = bb in all6D, simp_all)
-  apply (drule imp2D)
-    apply blast
-   apply (metis assns_agrees)
-  apply (clarsimp, rule_tac x=h' and y=hJ' in ex2I, simp add: hsimps)
-  apply (rule conjI, erule assns_agreesE, subst agreesC, assumption)
-  apply (erule (1) mall5_imp2D, simp add: agreesC)
-  apply (drule rered_properties, auto)
-  done
-
-definition 
-  reCSL :: "(rname \<Rightarrow> assn) \<Rightarrow> assn \<Rightarrow> revent \<Rightarrow> assn \<Rightarrow> bool" 
-  ("_ \<turnstile>\<^sub>r\<^sub>e { _ } _ { _ }")
-  where
-    "\<Gamma> \<turnstile>\<^sub>r\<^sub>e {P} re {Q} \<equiv> (user_revent re) \<and> (\<forall>n s h. (s, h) \<Turnstile> P \<longrightarrow> resafe n re s h \<Gamma> Q)"
-
-lemma resafe_conseq : "\<lbrakk> resafe n re s h \<Gamma> Q; Q \<sqsubseteq> Q'\<rbrakk> \<Longrightarrow> resafe n re s h \<Gamma> Q'"
-    apply (induct n arbitrary: re s h, simp)
-  apply (clarsimp, simp add : implies_def)
-  apply (clarify, erule rered.cases, simp_all, clarsimp)
-   apply (drule_tac a = "hJ" and b = "hF" and c = "a" and d = "AnonyEvent C'" 
-          and e = "ab" and f = "bb" in all6_impD)
-    apply (metis rered.red_AnonyEvt)
-   apply (clarsimp, rule_tac x = "h'" and y = "hJ'" in ex2I, simp)
-  apply (drule_tac a = "hJ" and b = "hF" and c = "a" and d = "AnonyEvent C" 
-         and e = "s" and f = "h ++ hJ ++ hF" in all6_impD)
-   apply (metis fst_conv rered.red_BasicEvt)
-  apply (clarsimp, rule_tac x = "h'" and y = "hJ'" in ex2I, simp)
-  done
-
-theorem rule_rEvtconseq : "\<lbrakk>\<Gamma> \<turnstile>\<^sub>r\<^sub>e {P} re {Q} ; P' \<sqsubseteq> P; Q \<sqsubseteq> Q' \<rbrakk> \<Longrightarrow> \<Gamma>  \<turnstile>\<^sub>r\<^sub>e {P'} re {Q'}"
-  by (meson implies_def reCSL_def resafe_conseq)
-
-theorem rule_re_equiv: "\<lbrakk> \<Gamma> \<turnstile>\<^sub>r\<^sub>e {P} re {Q}; P \<equiv>\<^sub>S\<^sub>L P'; Q \<equiv>\<^sub>S\<^sub>L Q' \<rbrakk> \<Longrightarrow>  \<Gamma> \<turnstile>\<^sub>r\<^sub>e {P'} re {Q'}"
-  by (simp add: assn_equiv_symmetry equiv_implies rule_rEvtconseq)
-
-lemma resafe_res:
- "\<lbrakk>resafe n (rs, e) s h (\<Gamma>(r := R)) Q; wf_revent (rs, e); r \<notin> set rs;
-   disjoint (fvA R) (wrREv (rs, e)) \<rbrakk> \<Longrightarrow> (\<forall>hR. r \<notin> relocked (rs, e) \<longrightarrow> disjoint (dom h) (dom hR) 
-     \<longrightarrow> (s,hR) \<Turnstile> R \<longrightarrow> resafe n (r # rs, e) s (h ++ hR) \<Gamma> (Q ** R))
-   \<and> (r \<in> relocked (rs, e) \<longrightarrow> resafe n (r # rs, e) s h \<Gamma> (Q ** R))"
-  apply (induct n arbitrary: e s h, simp, clarsimp)
-  apply (rule conjI, clarify)
-   apply (rule conjI) apply auto[1]
-  apply (rule conjI)
-    apply (metis disjoint_simps(4) dom_map_add map_add_assoc reaborts.simps snd_conv)
-   apply (rule conjI, simp add: le_supI2 reaccesses_def)
-   apply (clarify, frule rered_properties, clarsimp)
-   apply (subgoal_tac "a = r # rs", simp)
-    apply (case_tac "r \<in> set (rellocked (rs, b))", simp add: rellocked_def)
-  apply (drule_tac a = "hJ ++ hR" and b = "hF" and c = rs and d = b and e = aa
-          and f = "ba" in all6_impD, simp add: hsimps)
-  apply (meson re_equiv3)
-     apply (drule imp2D, subst sat_envs_expand [where r=r], simp_all add: relocked_def elocked_eq)
-       apply (subgoal_tac "wf_revent (r # rs, e)")
-        apply (subgoal_tac "wf_revent (a, b)", simp add: wf_revent_def)
-         apply (simp add: distinct_list_minus wf_event_distinct_locked) 
-        apply (simp add: red_wf_revent, simp add: wf_revent_def)
-      apply (intro exI conjI, simp, simp_all add: envs_upd hsimps relocked_def)
-     apply (clarsimp, rule_tac x = "h'" and y = "hJ'" in ex2I, simp add: envs_removeAll_irr)
-     apply (drule (1) mall3_imp2D)
-  using red_wf_revent re_equiv3 apply blast
-     apply (simp add: relocked_def elocked_eq, drule mimpD)
-      apply (meson disjoint_search(4) re_equiv3 rered_properties, simp)
-    apply (drule_tac a="hJ" and b="hR ++ hF" and c = rs and d = b and e = aa
-          and f = "ba" in all6_impD, simp add: hsimps)
-  using re_equiv3 apply blast
-    apply (drule imp2D, simp add: rellocked_def envs_upd(1)) apply auto[1]
-apply (clarsimp, rule_tac x = "h' ++ hR" and y = "hJ'" in ex2I, simp add: hsimps)
-    apply (rule conjI, simp add: envs_upd(1) rellocked_def relocked_eq)
-     apply (drule (1) mall3_imp2D)
-  using red_wf_revent re_equiv3 apply blast
-    apply (drule mimpD)
-     apply (meson disjoint_search(1) disjoint_search(2) re_equiv3 rered_properties)
-    apply (simp add: rellocked_def elocked_def)
-    apply (drule_tac a = "hR" in all_imp2D)
-  using disjoint_commute apply blast
-     apply (metis agrees_minusD assn_agrees disjoint_commute snd_eqD wrREv_def)
-
-    apply (simp add: map_add_commute)
-  using rered.simps apply auto[1]
-  apply (clarsimp, rule conjI) apply auto[1]
-  apply (rule conjI, simp add: reaborts_equiv)
-  apply (rule conjI, simp add: reaccesses_def)
-  apply (clarify, frule rered_properties, clarsimp)
-  apply (subgoal_tac "a = r # rs", simp)
-    apply (drule_tac a="hJ" and b=" hF" and c = rs and d = b and e = aa
-          and f = "ba" in all6_impD)
-  using re_equiv3 apply blast
-   apply (drule imp2D, simp add: envs_removeAll2 envs_upd(2) rellocked_def elocked_eq, simp)
-   apply (clarsimp, drule (1) mall3_imp2D)
-  using red_wf_revent re_equiv3 apply blast
-   apply (drule mimpD, meson disjoint_search(4) re_equiv3 rered_properties)
-   apply (case_tac "r \<in> set (rellocked (rs, b))", simp add: rellocked_def)
-    apply (intro exI conjI, simp+)
-     apply (simp add: envs_removeAll2 envs_upd(2), simp add: relocked_def elocked_eq)
-  apply (subst (asm) sat_envs_expand [where r=r]) back
-      apply (simp_all add: rellocked_def relocked_def elocked_eq)
-    apply (simp add: wf_revent_def)
-  using distinct_list_minus wf_event_distinct_locked apply blast
-   apply (clarsimp, drule (2) all_imp2D, rule_tac x = "h' ++ h1" and y = " h2" in ex2I, 
-        simp add: hsimps envs_upd)
-  by (metis fst_conv re_invres)
-
-lemma resafe_res_empty : "esafe n e s h \<Gamma> Q \<Longrightarrow> resafe n ([], e) s h \<Gamma> Q"
-  apply (induct n arbitrary: e s h, simp, clarsimp)
-  apply (rule conjI, simp add: reaborts_equiv)
-  apply (rule conjI, simp add: reaccesses_def, clarsimp)
-  apply (subgoal_tac "a = []", simp)
-   apply (drule_tac a = "hJ" and b = "hF" and c = "b" and d = "aa" and e = "ba" in all5_impD)
-  apply (meson re_equiv2)
-    apply (drule imp2D, simp add: rellocked_def, simp, clarsimp)
-   apply (rule_tac x = h' and y = hJ' in ex2I, simp add: rellocked_def)
-  by (metis fst_conv re_invres)
-
-theorem rule_re_empty : "\<Gamma> \<turnstile>\<^sub>e { P } e { Q } \<Longrightarrow> \<Gamma> \<turnstile>\<^sub>r\<^sub>e { P } ([], e) { Q }"
-  by (simp add: eCSL_def reCSL_def user_revent_def resafe_res_empty)
-
-lemma rule_re1 : "\<lbrakk> \<Gamma>(r := R) \<turnstile>\<^sub>r\<^sub>e {P} (rs, e) {Q} ; disjoint (fvA R) (wrREv (rs, e)); r \<notin> set rs \<rbrakk> 
-  \<Longrightarrow> \<Gamma> \<turnstile>\<^sub>r\<^sub>e  {P ** R} (r # rs, e) {Q ** R}"
-  apply (clarsimp simp add: reCSL_def)
-  apply (rule conjI, simp add: user_revent_def, clarsimp)
-  apply (drule_tac a = n and b = s and c = h1 in all3_impD, simp)
-  by (simp add: resafe_res user_reventD)
-
-theorem rule_re : 
-    "\<lbrakk>(update_list \<Gamma> \<G> rs) \<turnstile>\<^sub>e {P} e {Q} ;disjoint (fvA (Aistar (map \<G> rs))) (wrEv e); distinct rs\<rbrakk> 
-    \<Longrightarrow> \<Gamma> \<turnstile>\<^sub>r\<^sub>e {P ** (Aistar (map \<G> rs))} (rs, e) {Q ** (Aistar (map \<G> rs))}"
-  apply (induct rs arbitrary: \<Gamma>, rule_tac P = "P" and Q = "Q" in rule_re_equiv)
-     apply (simp add: rule_re_empty, simp, simp add: assn_equiv_def, simp add: assn_equiv_def)
-  apply (drule_tac a = "\<Gamma>(a := \<G> a)" in mall_impD, clarsimp)
-  apply (rule_tac P = "(P ** Aistar (map \<G> rs)) ** \<G> a" and Q = "(Q ** Aistar (map \<G> rs)) ** \<G> a"
-  in rule_re_equiv, rule rule_re1, simp, simp add: wrREv_def, simp)
-   apply (meson Aistar_equiv) apply (meson Aistar_equiv)
-  done
-
-lemma resafe_frame:
- "\<lbrakk> resafe n re s h J Q; 
-    disjoint (dom h) (dom hR);
-    disjoint (fvA R) (wrREv re);
-    (s,hR) \<Turnstile> R\<rbrakk>
-  \<Longrightarrow> resafe n re s (h ++ hR) J (Q ** R)"
-  apply (induct n arbitrary: re s h hR, simp, clarsimp)
-  apply (rule conjI, clarify, fast)
-  apply (rule conjI, clarify)
- (* no aborts *)
-   apply (drule_tac a="hR ++ hF" in all_impD, simp, simp add: hsimps)
-(* accesses *)
-  apply (rule conjI, erule order_trans, simp)
-(* step *)
-  apply (clarify, frule rered_properties, clarsimp)
-  apply (drule_tac a="hJ" and b="hR ++ hF" and c = aa and d = ba and e = ab and f = bb in all6D)
-  apply (drule imp3D, simp_all)
-    apply (metis map_add_assoc map_add_commute)
-  apply force
-  apply (clarsimp, rule_tac y="hJ'" and x="h' ++ hR" in ex2I, clarsimp simp add: hsimps)
-  apply (subst map_add_commute, simp add: hsimps)
-  apply (drule mall5D, erule mimp4D, simp_all add: hsimps)
- apply (erule (1) disjoint_search)
-  apply (subst assn_agrees, simp_all, fastforce)
-  done
-
-
-theorem rerule_frame:
- "\<lbrakk> \<Gamma> \<turnstile>\<^sub>r\<^sub>e {P} re {Q} ; disjoint (fvA R) (wrREv re) \<rbrakk>
-  \<Longrightarrow> \<Gamma> \<turnstile>\<^sub>r\<^sub>e {P ** R} re {Q ** R}"
-  by (auto simp add: reCSL_def intro: resafe_frame)
-
 subsection \<open>specification and proof rules for event systems\<close>
 
 primrec 
@@ -426,14 +217,14 @@ lemma essafe_conseq : "\<lbrakk> essafe n es s h \<Gamma> Q; Q \<sqsubseteq> Q'\
   apply (induct n arbitrary: es s h, simp)
   apply (clarsimp, simp add : implies_def)
   apply (erule esred.cases, simp_all, clarify)
-    apply (drule_tac a = "hJ" and b = "hF" and c = "EvtSeq (ab, bb) res" 
+    apply (drule_tac a = "hJ" and b = "hF" and c = "EvtSeq e' esa" 
           and d = "a" and e = "b" in all5_impD)
      apply (metis esred.red_EvtSeq1)
     apply (clarsimp, rule_tac x = "h'" and y = "hJ'" in ex2I, simp)
    apply (drule_tac a = "hJ" and b = "hF" and c = "es'" and d = "a" and e = "b" in all5_impD)
     apply (metis esred.red_EvtSeq2)
    apply (clarsimp, rule_tac x = "h'" and y = "hJ'" in ex2I, simp)
-  apply (drule_tac a = "hJ" and b = "hF" and c = "EvtSeq re' (EvtSys revts)" and d = "a" 
+  apply (drule_tac a = "hJ" and b = "hF" and c = "EvtSeq e' (EvtSys evts)" and d = "a" 
         and e = "b" in all5_impD)
    apply (metis esred.red_EvtSet)
   apply (clarsimp, rule_tac x = "h'" in exI, simp)
@@ -445,105 +236,79 @@ theorem rule_esconseq : "\<lbrakk>\<Gamma> \<turnstile>\<^sub>e\<^sub>s {P} es {
 theorem rule_es_equiv : "\<lbrakk>\<Gamma> \<turnstile>\<^sub>e\<^sub>s {P} es {Q};  P' \<equiv>\<^sub>S\<^sub>L P; Q \<equiv>\<^sub>S\<^sub>L Q' \<rbrakk> \<Longrightarrow> \<Gamma>  \<turnstile>\<^sub>e\<^sub>s {P'} es {Q'}"
   using equiv_implies rule_esconseq by blast
 
-(*
-lemma essafe_EvtSeq :"\<lbrakk>resafe n re s h \<Gamma> Q;
-        \<forall>m s' h'. m \<le> n \<and> (s', h') \<Turnstile> (Q ** (Aistar (map \<Gamma> (esllocked esys)))) 
-                \<longrightarrow> essafe m esys s' h' \<Gamma> R\<rbrakk> 
-      \<Longrightarrow>  essafe n (EvtSeq re esys) s h \<Gamma> R"
-  apply (induct n arbitrary: re s h, simp, clarsimp)
-  apply (rule conjI, clarsimp)
-   apply (erule esaborts.cases, simp_all, clarsimp)
-  apply (clarsimp, erule esred.cases, simp_all)
-   apply (clarify, drule_tac a = hJ and b = hF and c = ac and d = bc and e = aa and f= ba in all6_impD)
-    apply blast
-   apply (clarsimp, rule_tac x = "h'" and y = "hJ'" in ex2I, simp)
-  apply (clarify, simp add: rellocked_def)
-  apply (drule_tac a = Map.empty and b = "hJ ++hF" and c = ac and d = "AnonyEvent Cskip" and e = aa and f= ba in all6_impD)
-   apply (metis empty_map_add map_add_assoc, simp, clarsimp)
-  apply (rule_tac x = "h' ++ hJ" and y = "hJ'" in ex2I, simp)
-  apply (rule conjI)
-  apply (metis map_add_assoc map_add_commute)
-  apply (rule conjI)
-   apply (metis disjoint_commute)
-  apply (rule conjI, simp add: esllocked_def)
-  done
-*)
-
-lemma essafe_EvtSeq :"\<lbrakk>resafe n re s h \<Gamma> Q; user_esys esys;
+lemma essafe_EvtSeq :"\<lbrakk>esafe n e s h \<Gamma> Q; user_esys esys;
         \<forall>m s' h'. m \<le> n \<and> (s', h') \<Turnstile> Q  \<longrightarrow> essafe m esys s' h' \<Gamma> R\<rbrakk> 
-      \<Longrightarrow>  essafe n (EvtSeq re esys) s h \<Gamma> R"
-  apply (induct n arbitrary: re s h, simp, clarsimp)
-  apply (rule conjI, clarsimp)
+      \<Longrightarrow>  essafe n (EvtSeq e esys) s h \<Gamma> R"
+  apply (induct n arbitrary: e s h, simp, clarsimp)
+  apply (rule conjI)
   using esaborts.simps apply auto[1]
   apply (clarsimp, erule esred.cases, simp_all)
-   apply (metis prod.collapse)
-  apply (drule_tac a = Map.empty and b = "hJ ++hF" and c = "fst re'" and d = "AnonyEvent Cskip" 
-        and e = aa and f= ba in all6_impD)
+   apply meson
+  apply (drule_tac a = Map.empty and b = "hJ ++hF" and c = "AnonyEvent Cskip" 
+        and d = a and e = b in all5_impD)
    apply force
-  apply (simp add: rellocked_def, clarsimp)
+  apply (simp add: ellocked_def, clarsimp)
   apply (rule_tac x = h' and y = hJ' in ex2I, simp)
   by (smt (verit) bot_nat_0.extremum_unique essafe.simps(1) le_SucE le_boolD 
-      lift_Suc_antimono_le linorder_linear not_less_eq_eq resafe.simps(2) snd_conv)
+      lift_Suc_antimono_le linorder_linear not_less_eq_eq esafe.simps(2) snd_conv)
 
 
-theorem rule_EvtSeq :"\<lbrakk>\<Gamma> \<turnstile>\<^sub>r\<^sub>e {P} re {Q};
-                 \<Gamma> \<turnstile>\<^sub>e\<^sub>s {Q } esys {R}\<rbrakk> 
+theorem rule_EvtSeq :"\<lbrakk>\<Gamma> \<turnstile>\<^sub>e {P} re {Q}; \<Gamma> \<turnstile>\<^sub>e\<^sub>s {Q } esys {R}\<rbrakk> 
                 \<Longrightarrow> \<Gamma> \<turnstile>\<^sub>e\<^sub>s {P} (EvtSeq re esys) {R}"
-  by (auto simp add: reCSL_def esCSL_def intro!: essafe_EvtSeq)
+  by (auto simp add: eCSL_def esCSL_def intro!: essafe_EvtSeq)
 
-definition get_int_pre :: "state \<Rightarrow> revent set \<Rightarrow> (revent \<Rightarrow> assn) \<Rightarrow> bool"
-  where "get_int_pre \<sigma> es Pre \<equiv> \<forall> re \<in> es.  \<sigma> \<Turnstile> (Pre re)" 
+definition get_int_pre :: "state \<Rightarrow> event set \<Rightarrow> (event \<Rightarrow> assn) \<Rightarrow> bool"
+  where "get_int_pre \<sigma> es Pre \<equiv> \<forall>e \<in> es.  \<sigma> \<Turnstile> (Pre e)" 
 
-definition get_union_post :: "state \<Rightarrow> revent set \<Rightarrow> (revent \<Rightarrow> assn) \<Rightarrow> bool"
-  where "get_union_post \<sigma> es Post \<equiv>  \<exists>re \<in> es. \<sigma> \<Turnstile> (Post re)" 
+definition get_union_post :: "state \<Rightarrow> event set \<Rightarrow> (event \<Rightarrow> assn) \<Rightarrow> bool"
+  where "get_union_post \<sigma> es Post \<equiv>  \<exists>e \<in> es. \<sigma> \<Turnstile> (Post e)" 
 
-lemma pre_conj : "\<lbrakk> \<forall>re \<in> es. P \<sqsubseteq> (Pre re) ; \<sigma> \<Turnstile> P \<rbrakk> \<Longrightarrow> get_int_pre \<sigma> es Pre"
+lemma pre_conj : "\<lbrakk> \<forall>e \<in> es. P \<sqsubseteq> (Pre e) ; \<sigma> \<Turnstile> P \<rbrakk> \<Longrightarrow> get_int_pre \<sigma> es Pre"
   using get_int_pre_def implies_def by blast
 
-lemma post_dconj : "\<lbrakk>\<forall>re\<in>es. (Post re) \<sqsubseteq> Q; get_union_post \<sigma> es Post\<rbrakk> \<Longrightarrow> \<sigma> \<Turnstile> Q"
+lemma post_dconj : "\<lbrakk>\<forall>e \<in> es. (Post e) \<sqsubseteq> Q; get_union_post \<sigma> es Post\<rbrakk> \<Longrightarrow> \<sigma> \<Turnstile> Q"
   using get_union_post_def implies_def by blast
 
-lemma essafe_EvtSys : "\<lbrakk> \<forall> re \<in> es. user_revent re \<and> (\<forall>s h. (s, h) \<Turnstile> (Pre re) 
-                        \<longrightarrow> resafe n re s h \<Gamma> (Post re)); 
-                         \<forall> re \<in> es. (Post re) \<sqsubseteq> Q; get_int_pre (s, h) es Pre;
-                         \<forall> re1 re2. re1 \<in> es \<and> re2 \<in> es \<longrightarrow> Post re1 \<sqsubseteq> Pre re2\<rbrakk>
-                        \<Longrightarrow>  essafe n (EvtSys es) s h \<Gamma> Q"
+lemma essafe_EvtSys : "\<lbrakk> \<forall>e \<in> es. user_event e \<and> (\<forall>s h. (s, h) \<Turnstile> (Pre e) 
+                        \<longrightarrow> esafe n e s h \<Gamma> (Post e)); 
+                         \<forall> e \<in> es. (Post e) \<sqsubseteq> Q; get_int_pre (s, h) es Pre;
+                         \<forall> e1 e2. e1 \<in> es \<and> e2 \<in> es \<longrightarrow> Post e1 \<sqsubseteq> Pre e2\<rbrakk>
+                        \<Longrightarrow> essafe n (EvtSys es) s h \<Gamma> Q"
   apply (induct n arbitrary: s h, simp, simp)
   apply (rule conjI, clarsimp)
    apply (erule esaborts.cases, simp_all)
-   apply (drule_tac x = "re" in Set.bspec, simp) apply auto
-   apply (drule_tac a = "aa" and b = "h" in all2_impD)
-  using get_int_pre_def apply blast apply blast
-  apply (erule esred.cases, simp_all)
-  apply (frule_tac x = "re" in Set.bspec, simp) apply auto
+  using get_int_pre_def apply fastforce
+  apply (clarsimp, erule esred.cases, simp_all)
+  apply (frule_tac x = "e" in Set.bspec, simp) apply auto
   apply (drule_tac a = "s" and b = "h" in all2_impD)
-   apply (simp add: get_int_pre_def)
-  apply ( drule_tac a = "hJ" and b = "hF" and c = "ab" and d = "bb" and e = "a" and f = "b" in all6_impD)
+   apply (simp add: get_int_pre_def, clarify)
+  apply (drule_tac a = "hJ" and b = "hF" and c = "e'" and d = "a" and e = "b" in all5_impD)
    apply blast
   apply (drule imp2D, simp, simp, clarsimp)
   apply (rule_tac x = h' in exI, simp)
-  apply (rule_tac Q = "Post (aa, ba)" in essafe_EvtSeq, simp, simp)
+  apply (rule_tac Q = "Post e" in essafe_EvtSeq, simp, simp)
   apply (clarsimp, drule_tac a = "s'" and b = "h'a" in mall2_impD, clarsimp)
-   apply (drule_tac x = "(ac, b)" in Set.bspec, simp) apply auto[1]
-  apply (drule_tac a = "sa" and b = "ha" in all2_impD, simp)
-   apply (rule_tac n = "Suc n" in resafe_mon, simp, simp)
+   apply (drule_tac x = "ea" in Set.bspec, simp, clarsimp)
+   apply (drule_tac a = "sa" and b = "ha" in all2_impD, simp)
+   apply (rule_tac n = "Suc n" in esafe_mon, simp, simp)
   apply (drule mimpD)
-  apply (metis pre_conj prod.collapse) 
+  apply (metis pre_conj)
   using essafe_mon by auto
 
-theorem rule_EvtSys :  "\<lbrakk> \<forall> re \<in> es. \<Gamma> \<turnstile>\<^sub>r\<^sub>e {(Pre re)} re {Post re};
-                         \<forall> re \<in> es. P \<sqsubseteq> Pre re;
-                         \<forall> re \<in> es. (Post re) \<sqsubseteq> Q;
-                         \<forall> re1 re2. re1 \<in> es \<and> re2 \<in> es \<longrightarrow> Post re1 \<sqsubseteq> Pre re2\<rbrakk>
+
+theorem rule_EvtSys :  "\<lbrakk>\<forall>e \<in> es. \<Gamma> \<turnstile>\<^sub>e {(Pre e)} e {Post e};
+                         \<forall>e \<in> es. P \<sqsubseteq> Pre e;
+                         \<forall>e \<in> es. (Post e) \<sqsubseteq> Q;
+                         \<forall>e1 e2. e1 \<in> es \<and> e2 \<in> es \<longrightarrow> Post e1 \<sqsubseteq> Pre e2\<rbrakk>
                         \<Longrightarrow> \<Gamma> \<turnstile>\<^sub>e\<^sub>s {P} (EvtSys es) {Q}"
-  apply (simp add: esCSL_def reCSL_def, clarsimp)
+  apply (simp add: esCSL_def eCSL_def, clarsimp)
   apply (rule essafe_EvtSys, simp_all)
   by (simp add: pre_conj)
 
-definition all_Aemp :: "revent \<Rightarrow> assn"
+definition all_Aemp :: "event \<Rightarrow> assn"
   where "all_Aemp = (\<lambda>x. Aemp)"
 
-corollary rule_EvtSys' :  " \<forall> re \<in> es. \<Gamma> \<turnstile>\<^sub>r\<^sub>e {Aemp} re {Aemp}
+corollary rule_EvtSys' :  " \<forall> re \<in> es. \<Gamma> \<turnstile>\<^sub>e {Aemp} re {Aemp}
                         \<Longrightarrow> \<Gamma> \<turnstile>\<^sub>e\<^sub>s {Aemp} (EvtSys es) {Aemp}"
   apply (rule_tac Pre = "all_Aemp" and Post = "all_Aemp" in rule_EvtSys, simp_all add: all_Aemp_def)
   by (simp_all add: implies_def)
@@ -578,253 +343,10 @@ theorem esrule_frame:
   \<Longrightarrow> \<Gamma> \<turnstile>\<^sub>e\<^sub>s {P ** R} es {Q ** R}"
   by (auto simp add: esCSL_def intro: essafe_frame)
 
-subsection \<open>specification and proof rules for resource event systems\<close>
-
-primrec 
-  ressafe :: "nat \<Rightarrow> resys \<Rightarrow> stack \<Rightarrow> heap \<Rightarrow> (rname \<Rightarrow> assn) \<Rightarrow> assn \<Rightarrow> bool"
-where
-  "ressafe 0 res s h \<Gamma> Q = True"
-| "ressafe (Suc n) res s h \<Gamma> Q = (
- (\<forall>hF. disjoint (dom h) (dom hF) \<longrightarrow> \<not> resaborts res (s, h ++ hF))
-\<and> (resaccesses res s \<subseteq> dom h)
-\<and> (\<forall>hJ hF res' \<sigma>' x x' actk. 
-      (res, (s, h ++ hJ ++ hF), x) -res-actk\<rightarrow> (res', \<sigma>', x')
-    \<longrightarrow> (s, hJ) \<Turnstile> envs \<Gamma> (resllocked res') (resllocked res)
-    \<longrightarrow> (disjoint (dom h) (dom hJ) \<and> disjoint (dom h) (dom hF) \<and> disjoint (dom hJ) (dom hF))
-    \<longrightarrow> (\<exists>h' hJ'.
-            snd \<sigma>' = h' ++ hJ' ++ hF
-          \<and> disjoint (dom h') (dom hJ') \<and> disjoint (dom h') (dom hF) \<and> disjoint (dom hJ') (dom hF)
-          \<and> (fst \<sigma>', hJ') \<Turnstile> envs \<Gamma> (resllocked res) (resllocked res')
-          \<and> ressafe n res' (fst \<sigma>') h' \<Gamma> Q)))"
-
-lemma ressafe_mon:
-  "\<lbrakk> ressafe n res s h \<Gamma> Q; m \<le> n \<rbrakk> \<Longrightarrow> ressafe m res s h \<Gamma> Q"
-  apply (induct m arbitrary: res s n h, simp)
-  apply (case_tac n, clarify)
-  apply (simp only: safe.simps, clarsimp)
-  apply (drule_tac a = "hJ" and b = hF and c = aa and d = ba and e = ab and f = bb in all6_impD)
-   apply blast
-  apply (drule imp2D, simp, simp)
-  apply (clarsimp, rule_tac x="h'" in exI, rule_tac x="hJ'" in exI, simp)
-  done
-
-lemma ressafe_agrees: 
-    "\<lbrakk> ressafe n resys s h \<Gamma> Q ; 
-     agrees (fvREsv resys \<union> fvA Q \<union> fvAs \<Gamma>) s s' \<rbrakk>
-   \<Longrightarrow> ressafe n resys s' h \<Gamma> Q"
-  apply (induct n arbitrary: resys s s' h, simp, simp only: ressafe.simps, clarify)
-  apply (rule conjI, clarsimp)
-   apply (drule_tac resaborts_agrees, simp, fast, simp, simp)
-  apply (rule conjI, subst (asm) resaccesses_agrees, simp_all)
-  apply (clarify, drule_tac X = "fvREsv (a,b) \<union> fvAs \<Gamma> \<union> fvA Q" in resred_agrees,
-       simp (no_asm), fast, simp(no_asm), fast, clarify)
-  apply (drule_tac a = "hJ" and b = hF and c = aa and d = ba and e = s'a and f = bb in all6_impD)
-   apply auto[1]
-  apply (drule imp2D)
-  using assns_agrees apply blast
-  apply blast
-  apply (clarsimp, rule_tac x=h' and y=hJ' in ex2I, simp add: hsimps)
-  apply (rule conjI, erule assns_agreesE, subst agreesC, assumption)
-  apply (erule (1) mall5_imp2D, simp add: agreesC)
-  apply (drule resred_properties, auto)
-  done
-
-definition 
-  resCSL :: "(rname \<Rightarrow> assn) \<Rightarrow> assn \<Rightarrow> resys \<Rightarrow> assn \<Rightarrow> bool" 
-  ("_ \<turnstile>\<^sub>r\<^sub>e\<^sub>s { _ } _ { _ }")
-  where
-    "\<Gamma> \<turnstile>\<^sub>r\<^sub>e\<^sub>s {P} resys {Q} \<equiv> (user_resys resys) \<and> (\<forall>n s h. (s, h) \<Turnstile> P \<longrightarrow> ressafe n resys s h \<Gamma> Q)"
-
-lemma ressafe_conseq : "\<lbrakk> ressafe n res s h \<Gamma> Q; Q \<sqsubseteq> Q'\<rbrakk> \<Longrightarrow> ressafe n res s h \<Gamma> Q'"
-  apply (induct n arbitrary: res s h, simp)
-  apply (clarsimp, simp add : implies_def)
-  apply (erule resred.cases, simp_all, clarify)
-    apply (drule_tac a = "hJ" and b = "hF" and c = "a" and d = "EvtSeq (ad, bc) res" 
-          and e = "ab" and f = "bb" in all6_impD)
-     apply (meson resred.red_EvtSeq1)
-    apply (drule imp2D, simp, simp)
-    apply (clarsimp, rule_tac x = "h'" and y = "hJ'" in ex2I, simp)
-   apply (drule_tac a = "hJ" and b = "hF" and c = "a" 
-         and d = "ba"  and e = "ab" and f = "bb" in all6_impD)
-  apply (meson resred.red_EvtSeq2)
-   apply (clarsimp, rule_tac x = "h'" and y = "hJ'" in ex2I, simp, clarsimp)
-  apply ( drule_tac a = "hJ" and b = "hF" and c = "a" and d = "EvtSeq (ad, bc) (EvtSys revts)" and  
-          e = "ab" and f = "bb" in all6_impD)
-   apply (meson resred.red_EvtSet)
-  apply (simp add: resllocked_def, clarify, rule_tac x = "h'" in exI, simp)
-  done
-
-theorem rule_resconseq : "\<lbrakk>\<Gamma>  \<turnstile>\<^sub>r\<^sub>e\<^sub>s {P} res {Q};  P' \<sqsubseteq> P; Q \<sqsubseteq> Q' \<rbrakk> \<Longrightarrow> \<Gamma>  \<turnstile>\<^sub>r\<^sub>e\<^sub>s {P'} res {Q'}"
-  by (meson implies_def resCSL_def ressafe_conseq)
-
-theorem rule_res_equiv : "\<lbrakk>\<Gamma>  \<turnstile>\<^sub>r\<^sub>e\<^sub>s {P} res {Q};  P' \<equiv>\<^sub>S\<^sub>L P; Q \<equiv>\<^sub>S\<^sub>L Q' \<rbrakk> \<Longrightarrow> \<Gamma>  \<turnstile>\<^sub>r\<^sub>e\<^sub>s {P'} res {Q'}"
-  using equiv_implies rule_resconseq by blast
-
-lemma ressafe_res : 
-"\<lbrakk>ressafe n (rs, es) s h (\<Gamma>(r := R)) Q; wf_resys (rs, es); r \<notin> set rs;
-   disjoint (fvA R) (wrREsv (rs, es))\<rbrakk> \<Longrightarrow> 
-   (\<forall>hR. r \<notin> reslocked (rs, es) \<longrightarrow> disjoint (dom h) (dom hR) 
-     \<longrightarrow> (s,hR) \<Turnstile> R \<longrightarrow> ressafe n (r # rs, es) s (h ++ hR) \<Gamma> (Q ** R))
-   \<and> (r \<in> reslocked (rs, es) \<longrightarrow> ressafe n (r # rs, es) s h \<Gamma> (Q ** R))"
-  apply (induct n arbitrary: es s h, simp, clarsimp)
-  apply (rule conjI, clarify)
-   apply (rule conjI, simp add: resaborts_equiv, clarify)
-    apply (metis disjoint_simps(4) dom_map_add map_add_assoc)
-   apply (rule conjI, simp add: resaccesses_def, erule order_trans, simp)
-   apply (clarify, frule resred_properties, clarsimp)
-   apply (subgoal_tac "a = r # rs", simp)
-    apply (case_tac "r \<in> set (resllocked (rs, b))", simp add: resllocked_def)
-  apply (drule_tac a = "hJ ++ hR" and b = "hF" and c = rs and d = b and e = aa
-          and f = "ba" in all6_impD, simp add: hsimps)
-  using res_equiv3 apply blast
-     apply (drule imp2D, subst sat_envs_expand [where r=r], simp_all add: resllocked_def)
-       apply (simp add: reslocked_def eslocked_eq)
-      apply (subgoal_tac "wf_resys (r # rs, es)")
-       apply (subgoal_tac "wf_resys (a, b)")
-        apply (simp add: wf_resys_def)
-        apply (simp add: distinct_list_minus wf_esys_distinct_locked)
-  using red_wf_resys apply blast
-      apply (simp add: wf_resys_def)
-      apply (intro exI conjI, simp, simp_all add: envs_upd hsimps rellocked_def)
-  apply (metis envs_def list_minus_removeAll list_minus_removeAll2)
-     apply (clarsimp, rule_tac x = "h'" and y = "hJ'" in ex2I, simp add: envs_removeAll_irr)
-     apply (rule conjI, simp add: envs_def list_minus_removeAll)
-     apply (drule (1) mall3_imp2D)
-  using red_wf_resys res_equiv3 apply blast
-     apply (simp add: reslocked_def eslocked_eq, drule mimpD)
-      apply (meson disjoint_search(4) res_equiv3 resred_properties, simp)
-    apply (drule_tac a="hJ" and b="hR ++ hF" and c = rs and d = b and e = aa
-          and f = "ba" in all6_impD, simp add: hsimps)
-  using res_equiv3 apply blast
-    apply (drule imp2D)
-      apply (simp add: envs_removeAll_irr envs_upd(1))
-     apply auto[1]
-    apply (clarsimp, rule_tac x = "h' ++ hR" and y = "hJ'" in ex2I, simp add: hsimps)
-    apply (rule conjI, simp add: envs_upd(1) resllocked_def reslocked_eq)
-     apply (drule (1) mall3_imp2D)
-  using red_wf_resys res_equiv3 apply blast  
-    apply (simp add: reslocked_def eslocked_eq, drule mimpD)
-     apply (meson disjoint_search(1) disjoint_search(2) res_equiv3 resred_properties)
-    apply (drule_tac a = "hR" in all_imp2D)
-  using disjoint_commute apply blast
-     apply (metis (no_types, lifting) agrees_minusD assn_agrees 
-                disjoint_search(1) fst_conv res_equiv3 resred_properties)
-    apply (simp add: map_add_commute)
-  using resred.simps apply auto[1]
-  apply (clarsimp, rule conjI, simp add: resaborts_equiv)
-  apply (rule conjI, simp add: resaccesses_def)
-  apply (clarify, frule resred_properties, clarsimp)
-  apply (subgoal_tac "a = r # rs", simp)
-    apply (drule_tac a="hJ" and b=" hF" and c = rs and d = b and e = aa
-          and f = "ba" in all6_impD)
-  using res_equiv3 apply blast
-   apply (drule imp2D, simp add: envs_removeAll2 envs_upd(2) resllocked_def reslocked_eq, simp)
-   apply (clarsimp, drule (1) mall3_imp2D)
-  using red_wf_resys res_equiv3 apply blast
-   apply (drule mimpD, meson disjoint_search(4) res_equiv3 resred_properties)
-   apply (case_tac "r \<in> set (resllocked (rs, b))", simp add: resllocked_def)
-    apply (intro exI conjI, simp+)
-     apply (simp add: envs_removeAll2 envs_upd(2), simp add: reslocked_def eslocked_eq)
-   apply (subst (asm) sat_envs_expand [where r=r]) back
-      apply (simp_all add: resllocked_def reslocked_def eslocked_eq)
-    apply (simp add: wf_resys_def)
-  using distinct_list_minus wf_esys_distinct_locked apply blast
-   apply (clarsimp, drule (2) all_imp2D, rule_tac x = "h' ++ h1" and y = " h2" in ex2I, 
-        simp add: hsimps envs_upd)
-  using resred.simps by auto
-
-lemma ressafe_res_empty : "essafe n es s h \<Gamma> Q \<Longrightarrow> ressafe n ([], es) s h \<Gamma> Q"
-  apply (induct n arbitrary: es s h, simp, clarsimp)
-  apply (rule conjI, simp add: resaborts_equiv)
-  apply (rule conjI, simp add: resaccesses_def, clarsimp)
-  apply (subgoal_tac "a = []", simp)
-   apply (drule_tac a = "hJ" and b = "hF" and c = "b" and d = "aa" and e = "ba" in all5_impD)
-  apply (meson res_equiv2)
-   apply (simp add: res_equiv2)
-  apply (drule impD, simp add: resllocked_def)
-   apply (clarsimp, rule_tac x = "h'" and y = "hJ'" in ex2I, simp add: resllocked_def)
-  using resred.simps by auto
-
-lemma ressafe_res_empty' : "ressafe n ([], es) s h \<Gamma> Q \<Longrightarrow> essafe n es s h \<Gamma> Q"
-  apply (induct n arbitrary: es s h, simp, clarsimp)
-  apply (rule conjI, simp add: resaborts_equiv)
-  apply (rule conjI, simp add: resaccesses_def, clarsimp)
-  apply (drule_tac a = "hJ" and b = "hF" and c = "[]" and d = "es'" and e = "a" and f = "b" in all6_impD)
-  apply (metis res_equiv1)
-  apply (drule impD, simp add: resllocked_def, clarsimp)
-  apply (rule_tac x = "h'" and y = "hJ'" in ex2I, simp add: resllocked_def)
-  done
-
-lemma rule_res_empty : "\<Gamma> \<turnstile>\<^sub>e\<^sub>s { P } es { Q } \<Longrightarrow> \<Gamma> \<turnstile>\<^sub>r\<^sub>e\<^sub>s { P } ([], es) { Q}"
-  by (simp add: esCSL_def resCSL_def user_resys_def ressafe_res_empty)
-
-lemma rule_res1 : "\<lbrakk> \<Gamma>(r := R) \<turnstile>\<^sub>r\<^sub>e\<^sub>s {P} (rs, es) {Q} ; disjoint (fvA R) (wrREsv (rs, es)); r \<notin> set rs \<rbrakk> 
-  \<Longrightarrow> \<Gamma> \<turnstile>\<^sub>r\<^sub>e\<^sub>s  {P ** R} (r # rs, es) {Q ** R}"
-  apply (clarsimp simp add: resCSL_def)
-  apply (rule conjI, simp add: user_resys_def, clarsimp)
-  apply (drule_tac a = n and b = s and c = h1 in all3_impD, simp)
-  by (simp add: ressafe_res user_resysD)
-
-theorem rule_res : 
-    "\<lbrakk>(update_list \<Gamma> \<G> rs) \<turnstile>\<^sub>e\<^sub>s {P} es {Q} ;disjoint (fvA (Aistar (map \<G> rs))) (wrEsv es)
-    ; distinct rs\<rbrakk>  \<Longrightarrow> \<Gamma> \<turnstile>\<^sub>r\<^sub>e\<^sub>s {P ** (Aistar (map \<G> rs))} (rs, es) {Q ** (Aistar (map \<G> rs))}"
-  apply (induct rs arbitrary: \<Gamma>, simp, rule_tac P = P and Q = Q in rule_res_equiv)
-  apply (simp add: rule_res_empty, simp add: assn_equiv_def, simp add: assn_equiv_def)
-  apply (drule_tac a = "\<Gamma>(a := \<G> a)" in mall_impD, clarsimp)
-  apply (rule_tac P = "(P ** Aistar (map \<G> rs)) ** \<G> a" and Q = "(Q ** Aistar (map \<G> rs)) ** \<G> a"
-  in rule_res_equiv, rule rule_res1, simp, simp add: wrREsv_def, simp)
-   apply (meson Aistar_equiv assn_equiv_symmetry) apply (meson Aistar_equiv assn_equiv_symmetry)
-  done
-
-theorem rule_rEvtSeq : "\<lbrakk>(update_list \<Gamma> \<G> rs) \<turnstile>\<^sub>r\<^sub>e {P} re {Q};
-                         (update_list \<Gamma> \<G> rs) \<turnstile>\<^sub>e\<^sub>s {Q } esys {R};
-                         disjoint (fvA (Aistar (map \<G> rs))) (wrEsv (EvtSeq re esys)); distinct rs\<rbrakk>
-   \<Longrightarrow> \<Gamma> \<turnstile>\<^sub>r\<^sub>e\<^sub>s {P ** (Aistar (map \<G> rs))} (rs, (EvtSeq re esys)) {R ** (Aistar (map \<G> rs))}"
-  by (rule rule_res, simp_all add: rule_EvtSeq)
-
-theorem rule_rEvtSys :  "\<lbrakk>\<forall> re \<in> es. (update_list \<Gamma> \<G> rs) \<turnstile>\<^sub>r\<^sub>e {(Pre re)} re {Post re};
-                         \<forall> re \<in> es. (Post re) \<sqsubseteq> Q; \<forall> re \<in> es. P \<sqsubseteq> (Pre re); 
-                         \<forall> re1 re2. re1 \<in> es \<and> re2 \<in> es \<longrightarrow> Post re1 \<sqsubseteq> Pre re2;
-                        disjoint (fvA (Aistar (map \<G> rs))) (wrEsv (EvtSys es)); distinct rs\<rbrakk>
-                        \<Longrightarrow>  \<Gamma> \<turnstile>\<^sub>r\<^sub>e\<^sub>s {P ** (Aistar (map \<G> rs))} (rs, (EvtSys es)) 
-                                    {Q ** (Aistar (map \<G> rs))}"
-  by (rule rule_res, simp_all add: rule_EvtSys)
-
-
-lemma ressafe_frame:
- "\<lbrakk> ressafe n res s h J Q; 
-    disjoint (dom h) (dom hR);
-    disjoint (fvA R) (wrREsv res);
-    (s,hR) \<Turnstile> R\<rbrakk>
-  \<Longrightarrow> ressafe n res s (h ++ hR) J (Q ** R)"
-  apply (induct n arbitrary: res s h hR, simp, clarsimp)
-  apply (rule conjI, clarify)
- (* no aborts *)
-   apply (drule_tac a="hR ++ hF" in all_impD, simp, simp add: hsimps)
-(* accesses *)
-  apply (rule conjI, erule order_trans, simp)
-(* step *)
-  apply (clarify, frule resred_properties, clarsimp)
-  apply (drule_tac a="hJ" and b="hR ++ hF" and c = aa and d = ba and e = ab and f = bb in all6_impD)
-  apply (metis map_add_assoc map_add_commute)
-  apply (drule imp2D, simp)
-  apply auto[1]
-  apply (clarsimp, rule_tac y="hJ'" and x="h' ++ hR" in ex2I, clarsimp simp add: hsimps)
-  apply (subst map_add_commute, simp add: hsimps)
-  apply (drule mall5D, erule mimp4D, simp_all add: hsimps)
- apply (erule (1) disjoint_search)
-  using agrees_minusD assn_agrees disjoint_search(1) by blast
-
-theorem resrule_frame:
- "\<lbrakk> \<Gamma> \<turnstile>\<^sub>r\<^sub>e\<^sub>s {P} res {Q} ; disjoint (fvA R) (wrREsv res) \<rbrakk>
-  \<Longrightarrow> \<Gamma> \<turnstile>\<^sub>r\<^sub>e\<^sub>s {P ** R} res {Q ** R}"
-  by (auto simp add: resCSL_def intro: ressafe_frame)
-
 subsection \<open>specification and proof rules for parallel event systems\<close>
 
 primrec 
-  pessafe :: "nat \<Rightarrow> paresys \<Rightarrow> stack \<Rightarrow> heap \<Rightarrow> (rname \<Rightarrow> assn) \<Rightarrow> assn \<Rightarrow> bool"
-  where
+  pessafe :: "nat \<Rightarrow> paresys \<Rightarrow> stack \<Rightarrow> heap \<Rightarrow> (rname \<Rightarrow> assn) \<Rightarrow> assn \<Rightarrow> bool" where
   "pessafe 0 pes s h \<Gamma> Q = True"
 | "pessafe (Suc n) pes s h \<Gamma> Q =  (
  (\<forall>hF. disjoint (dom h) (dom hF) \<longrightarrow> \<not> pesaborts pes (s, h ++ hF))
@@ -837,7 +359,6 @@ primrec
           \<and> disjoint (dom h') (dom hJ') \<and> disjoint (dom h') (dom hF) \<and> disjoint (dom hJ') (dom hF)
           \<and> (fst \<sigma>', hJ') \<Turnstile> envs \<Gamma> (pesllocked pes) (pesllocked pes')
           \<and> pessafe n pes' (fst \<sigma>') h' \<Gamma> Q)))"
-
 definition 
   pesCSL :: "(rname \<Rightarrow> assn) \<Rightarrow> assn \<Rightarrow> paresys \<Rightarrow> assn \<Rightarrow> bool" 
   ("_ \<turnstile>\<^sub>p\<^sub>e\<^sub>s { _ } _ { _ }")
@@ -845,10 +366,10 @@ definition
     "\<Gamma> \<turnstile>\<^sub>p\<^sub>e\<^sub>s {P} pes {Q} \<equiv> (user_pesys pes) \<and> (\<forall>n s h. (s, h) \<Turnstile> P \<longrightarrow> pessafe n pes s h \<Gamma> Q)"
 
 lemma pessafe_conseq : "\<lbrakk> pessafe n pes s h \<Gamma> Q; Q \<sqsubseteq> Q'\<rbrakk> \<Longrightarrow> pessafe n pes s h \<Gamma> Q'"
-    apply (induct n arbitrary: pes s h, simp)
+  apply (induct n arbitrary: pes s h, simp)
   apply (clarsimp, simp add : implies_def)
   apply (erule pesred.cases, simp_all, clarsimp)
-  apply (drule_tac a = "hJ" and b = "hF" and c = "pesa[k := (ab, bb)]" 
+  apply (drule_tac a = "hJ" and b = "hF" and c = "pesa[k := es']" 
           and d = "a" and e = "b" in all5_impD)
   using pesred.red_Par apply blast
    apply (clarsimp, rule_tac x = "h'" and y = "hJ'" in ex2I, simp)
@@ -865,56 +386,46 @@ lemma envs_app' : "disjoint (set a) (set b) \<Longrightarrow> disjoint (set a) (
     \<Longrightarrow> envs \<Gamma> (a @ b @ c) (a @ b' @ c) = envs \<Gamma> b b'"
   by (simp add: envs_app(1) envs_app(2))
 
-lemma disjoint_locked_list_update : 
-        "\<lbrakk> \<forall>k'. k' < length l \<and> k' \<noteq> k \<longrightarrow> disjoint (reslocked re) (reslocked (l ! k'));
-        disjoint_locked_list l ; k < length l \<rbrakk>
-    \<Longrightarrow> disjoint_locked_list (l [k := re])"
-  apply (simp add: disjoint_locked_list_equiv, clarify)
-  apply (case_tac "k1 = k", simp)
-  apply (case_tac "k2 = k")
-   apply auto[1]
-  by simp
-
-lemma pesllocked_cancel : "\<lbrakk>disjoint_locked_list pes; pes ! k = res;
-             pes' = pes[k := res']; k < length pes\<rbrakk>
+lemma pesllocked_cancel : "\<lbrakk>disjoint_locked_list pes; pes ! k = es;
+             pes' = pes[k := es']; k < length pes\<rbrakk>
         \<Longrightarrow> envs \<Gamma> (pesllocked pes) (pesllocked pes')
-          = envs \<Gamma> (resllocked res) (resllocked res')"
+          = envs \<Gamma> (esllocked es) (esllocked es')"
   apply (simp add: peslocked_split)
   apply (rule envs_app')
     apply (metis disjoint_locked_with_property disjoint_search(1)
-              disjoint_with_take peslocked_def reslocked_eq)
+              disjoint_with_take peslocked_def eslocked_eq)
    apply (simp add: peslocked_eq disjoint_between_take_drop disjoint_locked_between_property)
-  by (metis disjoint_locked_with_property disjoint_with_drop peslocked_def reslocked_eq)
+  by (metis disjoint_locked_with_property disjoint_with_drop peslocked_def eslocked_eq)
 
 lemma pessafe_pesllocked_cancel :
-        "\<lbrakk> disjoint_locked_list pes; pes' = pes[k := res']; pes ! k = res; k < length pes;
-         \<forall>k'. k' < length pes \<and> k \<noteq> k' \<longrightarrow> disjoint (reslocked res') (reslocked (pes ! k'))\<rbrakk>
+        "\<lbrakk> disjoint_locked_list pes; pes' = pes[k := es']; pes ! k = es; k < length pes;
+         \<forall>k'. k' < length pes \<and> k \<noteq> k' \<longrightarrow> disjoint (eslocked es') (eslocked (pes ! k'))\<rbrakk>
         \<Longrightarrow> envs \<Gamma> (pesllocked pes') (pesllocked pes)
-          = envs \<Gamma> (resllocked res') (resllocked res)"
+          = envs \<Gamma> (esllocked es') (esllocked es)"
   apply (rule pesllocked_cancel, simp_all)
   using disjoint_locked_list_update apply blast
   by auto
 
 lemma pessafe: 
-" \<lbrakk>\<forall>k. k < length pes \<longrightarrow> ressafe n (pes ! k) s (hs ! k) \<Gamma> (Qs ! k);
+" \<lbrakk>\<forall>k. k < length pes \<longrightarrow> essafe n (pes ! k) s (hs ! k) \<Gamma> (Qs ! k);
    disjoint_heap_list hs; disjoint_locked_list pes;
    \<forall>k1 k2. k1 < length pes \<and> k2 < length pes \<and> k1 \<noteq> k2 
-          \<longrightarrow> disjoint (fvREsv (pes ! k1) \<union> fvA (Qs ! k1) \<union> fvAs \<Gamma>) (wrREsv (pes ! k2));
+          \<longrightarrow> disjoint (fvEsv (pes ! k1) \<union> fvA (Qs ! k1) \<union> fvAs \<Gamma>) (wrEsv (pes ! k2));
     length pes = length hs\<rbrakk>
    \<Longrightarrow> pessafe n pes s (hplus_list hs) \<Gamma> (Aistar Qs)"
   apply (induct n arbitrary: pes s hs, simp, clarsimp)
   apply (rule conjI, clarsimp, erule pesaborts.cases, clarsimp)
     apply (simp add: pessafe_noaborts, clarsimp)
-  apply (meson disjoint_list_equiv disjoint_search(2) disjoint_search(4) reswrites_accesses)
+  apply (meson disjoint_list_equiv disjoint_search(2) disjoint_search(4) eswrites_accesses)
   apply (clarsimp, erule pesred.cases, simp)
-  apply (frule_tac a = "k" in allD, clarsimp)
+  apply (frule_tac a = "k" in allD, clarify)
   apply (drule_tac a = "hJ" and b = "(hplus_list (hs[ k:= Map.empty]) ++ hF)"
-          and c = "ab" and d = "bb" and e = "a" and f = "b" in all6_impD)
+          and c = "es'" and d = "a" and e = "b"  in all5_impD)
   using pessafe_hsimps2 apply auto[1]
   apply (drule imp2D)
     apply (simp add: pessafe_pesllocked_cancel)
    apply (rule conjI, simp add: disjoint_hplus_list1)
-   apply (rule conjI, simp add: disjoint_hplus_list3 disjoint_hplus_list1 )
+   apply (rule conjI, simp add: disjoint_hplus_list3 disjoint_hplus_list1)
     apply (simp add: disjoint_hplus_list3)
    apply (metis (no_types, lifting) disjoint_search(1) 
           disjoint_simps(4) dom_map_add hplus_list_exchange)
@@ -926,12 +437,11 @@ lemma pessafe:
    apply (simp add: disjoint_hplus_list2)
   apply (rule conjI)
   apply (simp add: pesllocked_cancel)
-   apply (drule resred_properties)
-   apply (clarsimp, drule_tac a = "pesa[k := (ab, bb)]" and b = "a"
-                              and c = "hs[k := h']" in mall3_impD)
+   apply (drule esred_properties)
+   apply (clarsimp, drule_tac a = "pesa[k := es']" and b = "a" and c = "hs[k := h']" in mall3_impD)
    apply (clarsimp, case_tac "ka = k", simp, simp)
-   apply (rule_tac s = "s" in ressafe_agrees)
-    apply (rule_tac n = "Suc n" in ressafe_mon, simp, simp)
+   apply (rule_tac s = "s" in essafe_agrees)
+    apply (rule_tac n = "Suc n" in essafe_mon, simp, simp)
    apply (drule_tac a = "ka" and b = "k" in all2_impD, simp, simp)
    apply auto[1]
   apply (drule mimp4D)
@@ -954,40 +464,40 @@ lemma split_Aistar : "(s, h) \<Turnstile> Aistar Ps \<Longrightarrow> (\<exists>
   using disjoint_heap_with_equiv2 disjoint_hplus_list1 disjoint_search(1) apply blast
   using less_Suc_eq_0_disj by auto
 
-theorem rule_pes : " \<lbrakk>\<forall>k. k < length pes \<longrightarrow> \<Gamma>  \<turnstile>\<^sub>r\<^sub>e\<^sub>s  {Ps ! k} (pes ! k) {Qs ! k};
+theorem rule_pes : " \<lbrakk>\<forall>k. k < length pes \<longrightarrow> \<Gamma>  \<turnstile>\<^sub>e\<^sub>s  {Ps ! k} (pes ! k) {Qs ! k};
                   \<forall>k1 k2. k1 < length pes \<and> k2 < length pes \<and> k1 \<noteq> k2 
-                  \<longrightarrow> disjoint (fvREsv (pes ! k1) \<union> fvA (Qs ! k1) \<union> fvAs \<Gamma>) (wrREsv (pes ! k2));
+                  \<longrightarrow> disjoint (fvEsv (pes ! k1) \<union> fvA (Qs ! k1) \<union> fvAs \<Gamma>) (wrEsv (pes ! k2));
                   length pes = length Ps \<rbrakk> 
                   \<Longrightarrow> \<Gamma>  \<turnstile>\<^sub>p\<^sub>e\<^sub>s {Aistar Ps} pes {Aistar Qs}"
-  apply (simp add: resCSL_def pesCSL_def, clarify)
+  apply (simp add: esCSL_def pesCSL_def, clarify)
   apply (drule split_Aistar, clarify)
   apply (rule pessafe, simp_all)
-  apply (simp add: user_pesysD wf_peslocked)
+   apply (simp add: disjoint_locked_list_equiv user_esysD)
   by blast
 
 lemma List_Aemp_equiv : "Aistar (replicate n Aemp) \<equiv>\<^sub>S\<^sub>L Aemp"
   by (induct n, simp_all add: assn_equiv_def)
 
-theorem rule_pes' : " \<lbrakk>\<forall>k. k < length pes \<longrightarrow> \<Gamma>  \<turnstile>\<^sub>r\<^sub>e\<^sub>s  {Aemp} (pes ! k) {Aemp};
+theorem rule_pes' : " \<lbrakk>\<forall>k. k < length pes \<longrightarrow> \<Gamma>  \<turnstile>\<^sub>e\<^sub>s  {Aemp} (pes ! k) {Aemp};
                   \<forall>k1 k2. k1 < length pes \<and> k2 < length pes \<and> k1 \<noteq> k2 
-                  \<longrightarrow> disjoint (fvREsv (pes ! k1)  \<union> fvAs \<Gamma>) (wrREsv (pes ! k2))\<rbrakk> 
+                  \<longrightarrow> disjoint (fvEsv (pes ! k1)  \<union> fvAs \<Gamma>) (wrEsv (pes ! k2))\<rbrakk> 
                   \<Longrightarrow> \<Gamma>  \<turnstile>\<^sub>p\<^sub>e\<^sub>s {Aemp} pes {Aemp}"
   apply (rule_tac P = "Aistar (replicate (length pes) Aemp)" and Q = "Aistar (replicate (length pes)
-   Aemp)" in rule_pes_equiv, rule rule_pes, simp_all) apply blast
+   Aemp)" in rule_pes_equiv, rule rule_pes, simp_all)
+    apply blast
   by (simp_all add: assn_equiv_symmetry List_Aemp_equiv)
 
-
-corollary rule_pes2' : "\<lbrakk>\<Gamma>  \<turnstile>\<^sub>r\<^sub>e\<^sub>s {P1} res1 {Q1} ; \<Gamma>  \<turnstile>\<^sub>r\<^sub>e\<^sub>s {P2} res2 {Q2};
-           disjoint ((fvREsv res1) \<union> fvA Q1 \<union> fvAs \<Gamma>) (wrREsv res2);
-           disjoint ((fvREsv res2) \<union> fvA Q2 \<union> fvAs \<Gamma>) (wrREsv res1)\<rbrakk>
-           \<Longrightarrow> \<Gamma>  \<turnstile>\<^sub>p\<^sub>e\<^sub>s {Aistar [P1, P2]} [res1, res2] {Aistar [Q1, Q2]}"
+corollary rule_pes2' : "\<lbrakk>\<Gamma> \<turnstile>\<^sub>e\<^sub>s {P1} es1 {Q1} ; \<Gamma> \<turnstile>\<^sub>e\<^sub>s {P2} es2 {Q2};
+           disjoint ((fvEsv es1) \<union> fvA Q1 \<union> fvAs \<Gamma>) (wrEsv es2);
+           disjoint ((fvEsv es2) \<union> fvA Q2 \<union> fvAs \<Gamma>) (wrEsv es1)\<rbrakk>
+           \<Longrightarrow> \<Gamma>  \<turnstile>\<^sub>p\<^sub>e\<^sub>s {Aistar [P1, P2]} [es1, es2] {Aistar [Q1, Q2]}"
   apply (rule rule_pes, simp_all add: less_Suc_eq)
   by auto
 
-corollary rule_pes2 : "\<lbrakk>\<Gamma>  \<turnstile>\<^sub>r\<^sub>e\<^sub>s {P1} res1 {Q1} ; \<Gamma>  \<turnstile>\<^sub>r\<^sub>e\<^sub>s {P2} res2 {Q2};
-           disjoint ((fvREsv res1) \<union> fvA Q1 \<union> fvAs \<Gamma>) (wrREsv res2);
-           disjoint ((fvREsv res2) \<union> fvA Q2 \<union> fvAs \<Gamma>) (wrREsv res1)\<rbrakk>
-           \<Longrightarrow> \<Gamma>  \<turnstile>\<^sub>p\<^sub>e\<^sub>s {P1 ** P2} [res1, res2] {Q1 ** Q2}"
+corollary rule_pes2 : "\<lbrakk>\<Gamma>  \<turnstile>\<^sub>e\<^sub>s {P1} es1 {Q1} ; \<Gamma>  \<turnstile>\<^sub>e\<^sub>s {P2} es2 {Q2};
+           disjoint ((fvEsv es1) \<union> fvA Q1 \<union> fvAs \<Gamma>) (wrEsv es2);
+           disjoint ((fvEsv es2) \<union> fvA Q2 \<union> fvAs \<Gamma>) (wrEsv es1)\<rbrakk>
+           \<Longrightarrow> \<Gamma>  \<turnstile>\<^sub>p\<^sub>e\<^sub>s {P1 ** P2} [es1, es2] {Q1 ** Q2}"
   apply (rule_tac P = "Aistar [P1, P2]" and Q = "Aistar [Q1, Q2]" in rule_pesconseq)
   using rule_pes2' apply auto[1]
   by (simp_all add: implies_def)
@@ -1083,7 +593,7 @@ lemma rpessafe_res:
         apply (simp add: distinct_list_minus wf_pesys_distinct_locked)
   using red_wf_rpesys apply blast
       apply (simp add: wf_rpesys_def)
-      apply (intro exI conjI, simp, simp_all add: envs_upd hsimps rellocked_def)
+      apply (intro exI conjI, simp, simp_all add: envs_upd hsimps ellocked_def)
   apply (metis envs_def list_minus_removeAll list_minus_removeAll2)
      apply (clarsimp, rule_tac x = "h'" and y = "hJ'" in ex2I, simp add: envs_removeAll_irr)
      apply (rule conjI, simp add: envs_def list_minus_removeAll)
@@ -1118,7 +628,7 @@ apply (clarsimp, rule conjI, simp add: rpesaborts_equiv)
   apply (metis envs_removeAll2 envs_upd(2) fst_eqD rpesllocked_def rpeslocked_eq sndI, simp)
    apply (clarsimp, drule (1) mall3_imp2D)
   using red_wf_pesys rpes_equiv2 apply blast
-   apply (drule mimpD, meson disjoint_search(4) rpes_equiv3 resred_properties)
+   apply (drule mimpD, meson disjoint_search(4) rpes_equiv3 esred_properties)
    apply (case_tac "r \<in> set (rpesllocked (rs, b))", simp add: rpesllocked_def)
     apply (intro exI conjI, simp+)
      apply (simp add: envs_removeAll2 envs_upd(2), simp add: rpeslocked_def peslocked_eq)
