Event_Computation.thy
@@ -29,18 +29,6 @@ definition gets_e :: " econf \<Rightarrow> state" where
 definition getx_e :: "econf \<Rightarrow>  x" where
   "getx_e conf \<equiv> snd (snd conf)"
 
-
-type_synonym reconf = "revent \<times> state \<times> x"
-
-definition getspc_re :: " reconf \<Rightarrow> revent" where
-  "getspc_re conf \<equiv> fst conf"
-
-definition gets_re :: " reconf \<Rightarrow> state" where
-  "gets_re conf \<equiv> fst (snd conf)"
-
-definition getx_re :: "reconf \<Rightarrow>  x" where
-  "getx_re conf \<equiv> snd (snd conf)"
-
 type_synonym esconf = "esys \<times> state \<times> x"
 
 definition getspc_es :: " esconf \<Rightarrow>  esys" where
@@ -52,17 +40,6 @@ definition gets_es :: "esconf \<Rightarrow> state" where
 definition getx_es :: "esconf \<Rightarrow> x" where
   "getx_es conf \<equiv> snd (snd conf)"
 
-type_synonym resconf = "resys \<times> state \<times> x"
-
-definition getspc_res :: " resconf \<Rightarrow>  resys" where
-  "getspc_res conf \<equiv> fst conf"
-
-definition gets_res :: "resconf \<Rightarrow> state" where
-  "gets_res conf \<equiv> fst (snd conf)"
-
-definition getx_res :: "resconf \<Rightarrow> x" where
-  "getx_res conf \<equiv> snd (snd conf)"
-
 type_synonym pesconf = "paresys \<times> state \<times> x"
 
 definition getspc_pes :: "pesconf \<Rightarrow> paresys" where
@@ -73,7 +50,6 @@ definition gets_pes :: "pesconf \<Rightarrow> state" where
 
 definition getx_pes :: " pesconf \<Rightarrow>  x" where
   "getx_pes conf \<equiv> snd (snd conf)"
-
 
 type_synonym rpesconf = "rparesys \<times> state \<times> x"
 
@@ -100,68 +76,16 @@ inductive
 | red_BasicEvt: "\<lbrakk>bdenot guard (fst \<sigma>); x' = x(k:= BasicEvent (guard, C))\<rbrakk> \<Longrightarrow> 
                  (BasicEvent (guard, C), \<sigma>, x)-et-(EvtEnt (BasicEvent (guard, C)))\<sharp>k\<rightarrow> (AnonyEvent C, \<sigma>, x')"
 
-inductive 
-  rered :: "reconf \<Rightarrow> actk \<Rightarrow> reconf  \<Rightarrow> bool" ("_ -ret-_\<rightarrow> _" [81,81,81] 80)
-  where     
-  red_AnonyEvt: "red C \<sigma> C' \<sigma>' \<Longrightarrow> ((rs,(AnonyEvent C)), \<sigma>, x) -ret-(Cmd CMP)\<sharp>k\<rightarrow> ((rs, (AnonyEvent C')), \<sigma>', x)"
-| red_BasicEvt: "\<lbrakk>bdenot guard (fst \<sigma>); x' = x(k:= BasicEvent (guard, C))\<rbrakk> 
-                 \<Longrightarrow> ((rs ,(BasicEvent (guard, C))), \<sigma>, x)-ret-(EvtEnt (BasicEvent (guard, C)))\<sharp>k\<rightarrow> 
-                     ((rs ,(AnonyEvent C)), \<sigma>, x')"
-
-lemma re_invres : "(re, \<sigma>, x) -ret-actk\<rightarrow> (re', \<sigma>', x') \<Longrightarrow> fst re = fst re'"
-  by (erule rered.cases, simp_all)
-
-lemma re_equiv1 : "(e, \<sigma>, x) -et-actk\<rightarrow> (e', \<sigma>', x') \<Longrightarrow> ((r, e), \<sigma>, x) -ret-actk\<rightarrow> ((r, e'), \<sigma>', x')"
-  apply (erule ered.cases, simp add: rered.red_AnonyEvt)
-  apply (simp add: rered.red_BasicEvt)
-  done
-
-lemma re_equiv2 : "((r, e), \<sigma>, x) -ret-actk\<rightarrow> ((r, e'), \<sigma>', x') \<Longrightarrow> (e, \<sigma>, x) -et-actk\<rightarrow> (e', \<sigma>', x')"
-  apply (erule rered.cases, simp add: ered.red_AnonyEvt)
-   apply (simp add: ered.red_BasicEvt)
-  done
-
-lemma re_equiv3 : "((r, e), \<sigma>, x) -ret-actk\<rightarrow> ((r, e'), \<sigma>', x') \<Longrightarrow> ((r', e), \<sigma>, x) -ret-actk\<rightarrow> ((r', e'), \<sigma>', x')"
-  by (simp add: rered.simps)
-
 subsubsection \<open>Operational Semantics for event systems and resource event systems\<close>
 inductive
   esred :: "esconf \<Rightarrow> actk \<Rightarrow> esconf \<Rightarrow> bool" ("_ -es-_\<rightarrow> _" [81,81,81] 80)
   where
-  red_EvtSeq1: "(re, \<sigma>, x)-ret-actk\<rightarrow> (re', \<sigma>', x) \<Longrightarrow> snd re' \<noteq> (AnonyEvent Cskip) 
-                \<Longrightarrow> ((EvtSeq re res), \<sigma>, x) -es-actk\<rightarrow> ((EvtSeq re' res), \<sigma>', x)"
-| red_EvtSeq2: "\<lbrakk>(re, \<sigma>, x)-ret-actk\<rightarrow>(re', \<sigma>', x); snd re' = (AnonyEvent Cskip)\<rbrakk> \<Longrightarrow>
-                ((EvtSeq re res), \<sigma>, x) -es-atck\<rightarrow> (res, \<sigma>', x)"
-| red_EvtSet: " \<lbrakk>re \<in> revts; (re, \<sigma>, x)-ret-(EvtEnt evt)\<sharp>k\<rightarrow>(re', \<sigma>', x')\<rbrakk>  
-              \<Longrightarrow> ((EvtSys revts), \<sigma>, x) -es-(EvtEnt evt)\<sharp>k\<rightarrow> ((EvtSeq re' (EvtSys revts)), \<sigma>', x')"
-
-inductive
-  resred :: "resconf \<Rightarrow> actk \<Rightarrow> resconf \<Rightarrow> bool"("_ -res-_\<rightarrow> _" [81,81,81] 80)
-  where
-  red_EvtSeq1: "(re, \<sigma>, x)-ret-actk\<rightarrow> (re', \<sigma>', x) \<Longrightarrow> snd re' \<noteq> (AnonyEvent Cskip)
-           \<Longrightarrow> ((rs, (EvtSeq re res)), \<sigma>, x) -res-actk\<rightarrow> ((rs, (EvtSeq re' res)), \<sigma>', x)"
-| red_EvtSeq2: "\<lbrakk>(re, \<sigma>, x)-ret-actk\<rightarrow>(re', \<sigma>', x); snd re' = (AnonyEvent Cskip)\<rbrakk> \<Longrightarrow> 
-               ((rs, (EvtSeq re res)), \<sigma>, x) -res-atck\<rightarrow> ((rs, res), \<sigma>', x)"
-| red_EvtSet: "\<lbrakk>re \<in> revts; (re, \<sigma>, x)-ret-(EvtEnt evt)\<sharp>k\<rightarrow>(re', \<sigma>', x')\<rbrakk>  \<Longrightarrow> 
-               ((rs, (EvtSys revts)), \<sigma>, x) -res-(EvtEnt evt)\<sharp>k\<rightarrow> ((rs, (EvtSeq re' (EvtSys revts))), \<sigma>', x')"
-
-lemma res_invres : "(res, \<sigma>, x) -res-actk\<rightarrow> (res', \<sigma>', x') \<Longrightarrow> fst res = fst res'"
-  by (erule resred.cases, simp_all)
-
-lemma res_equiv1 : "(es, \<sigma>, x) -es-actk\<rightarrow>(es', \<sigma>', x') \<Longrightarrow> ((r,es), \<sigma>, x) -res-actk\<rightarrow>((r, es'), \<sigma>', x')"
-  apply (erule esred.cases, simp add: resred.red_EvtSeq1)
-   apply (simp add: resred.red_EvtSeq2)
-  apply (simp add: resred.red_EvtSet)
-  done
-
-lemma res_equiv2 : "((r,es), \<sigma>, x) -res-actk\<rightarrow>((r, es'), \<sigma>', x') \<Longrightarrow> (es, \<sigma>, x) -es-actk\<rightarrow>(es', \<sigma>', x')"
-  apply (erule resred.cases, simp add: esred.red_EvtSeq1)
-   apply (simp add: esred.red_EvtSeq2)
-  apply (simp add: esred.red_EvtSet)
-  done
-
-lemma res_equiv3 : "((r,es), \<sigma>, x) -res-actk\<rightarrow>((r, es'), \<sigma>', x') \<Longrightarrow> ((r',es), \<sigma>, x) -res-actk\<rightarrow>((r', es'), \<sigma>', x')"
-  by (simp add: resred.simps)
+  red_EvtSeq1: "(e, \<sigma>, x)-et-actk\<rightarrow> (e', \<sigma>', x) \<Longrightarrow> e' \<noteq> (AnonyEvent Cskip) 
+                \<Longrightarrow> ((EvtSeq e es), \<sigma>, x) -es-actk\<rightarrow> ((EvtSeq e' es), \<sigma>', x)"
+| red_EvtSeq2: "\<lbrakk>(e, \<sigma>, x)-et-actk\<rightarrow>(e', \<sigma>', x); e' = (AnonyEvent Cskip)\<rbrakk> \<Longrightarrow>
+                ((EvtSeq e es), \<sigma>, x) -es-atck\<rightarrow> (es, \<sigma>', x)"
+| red_EvtSet: " \<lbrakk>e \<in> evts; (e, \<sigma>, x)-et-(EvtEnt evt)\<sharp>k\<rightarrow>(e', \<sigma>', x')\<rbrakk>  
+              \<Longrightarrow> ((EvtSys evts), \<sigma>, x) -es-(EvtEnt evt)\<sharp>k\<rightarrow> ((EvtSeq e' (EvtSys evts)), \<sigma>', x')"
 
 subsubsection \<open>Operational Semantics for parallel event systems and resource parallel event systems\<close>
 
@@ -263,96 +187,6 @@ lemma eaborts_agrees[rule_format]:
   apply (simp add: aborts_Evt aborts_agrees)
   done
 
-subsection \<open>functions for resource event  \<close>   
-
-subsubsection \<open>locks that a resource event is currently holding \<close>
-
-definition
-  relocked :: "revent \<Rightarrow> rname set"
-  where
-  "relocked re = (elocked (snd re)) - (set (fst re))"
-
-definition 
-  rellocked :: "revent \<Rightarrow> rname list"
-  where
-  "rellocked re = list_minus (ellocked (snd re)) (fst re)"
-
-lemma relocked_eq: "relocked re = set (rellocked re)"
-  by (simp add: elocked_eq rellocked_def relocked_def)
-
-subsubsection \<open>memory accesses and memory writes a resource event performs in one step \<close>
-
-definition
-  reaccesses :: "revent \<Rightarrow> stack \<Rightarrow> nat set"
-  where
-  "reaccesses re s = eaccesses (snd re) s"
-
-definition 
-  rewrite :: "revent \<Rightarrow> stack \<Rightarrow> nat set"
-  where
-  "rewrite re s = ewrite (snd re) s"
-
-subsubsection \<open>A resource event aborts in a given state\<close>
-
-inductive
-  reaborts :: "revent \<Rightarrow> state \<Rightarrow> bool"
-  where
-  aborts_Evt: "aborts C \<sigma> \<Longrightarrow> reaborts (r, (AnonyEvent C)) \<sigma>"
-
-lemma reaborts_equiv : "reaborts re \<sigma> = eaborts (snd re) \<sigma>"
-  by (metis eaborts.simps eq_snd_iff reaborts.simps)
-
-subsubsection \<open>free variable of resource event\<close>
-
-definition
-  fvREv :: "revent \<Rightarrow> var set"
-  where
-  "fvREv re = fvEv (snd re)"
-
-subsubsection \<open>all variables may be updated by a event\<close>
-
-definition
-  wrREv :: "revent \<Rightarrow> var set"
-  where
-  "wrREv re = wrEv (snd re)"
-
-subsubsection \<open>Basic properties about resource event semantics\<close>
-
-lemma rewrites_accesses : "rewrite re s \<subseteq> reaccesses re s"
-  by (simp add: rewrite_def reaccesses_def ewrites_accesses)
-
-lemma rered_properties:
-  " (re, \<sigma>, x) -ret-actk\<rightarrow> (re', \<sigma>', x') \<Longrightarrow> fvREv re' \<subseteq> fvREv re \<and> wrREv re' \<subseteq> wrREv re \<and> agrees (- wrREv re) (fst \<sigma>') (fst \<sigma>)"
-  apply (erule rered.cases, simp_all add: fvREv_def wrREv_def)
-   apply (simp add: red_properties)
-  by (simp add: agrees_refl)
-
-lemma reaccesses_agrees:
-  "agrees (fvREv re) s s' \<Longrightarrow> reaccesses re s = reaccesses re s'"
-  apply (induct re arbitrary: s s', simp_all add: fvREv_def reaccesses_def)
-  by (simp add: eaccesses_agrees)
-
-lemma rewrites_agrees:
-  "agrees (fvREv re) s s' \<Longrightarrow> rewrite re s = rewrite re s'"
-  apply (induct re arbitrary: s s', simp_all add: fvREv_def rewrite_def)
-  by (simp add: ewrites_agrees)
-
-lemma rered_agrees[rule_format]:
-  "(re, \<sigma>, x) -ret-actk\<rightarrow> (re', \<sigma>', x') \<Longrightarrow> \<forall>X s. agrees X (fst \<sigma>) s \<longrightarrow> snd \<sigma> = h \<longrightarrow> fvREv re \<subseteq> X \<longrightarrow>
-    (\<exists>s' h'. (re, (s, h), x) -ret-actk\<rightarrow> (re', (s', h'), x') \<and> agrees X (fst \<sigma>') s' \<and> snd \<sigma>' = h')"
-    apply (induct re, simp_all)
-  apply (erule rered.cases, simp_all, clarsimp)
-   apply (metis fst_conv fvEv.simps(1) fvREv_def red_agrees rered.red_AnonyEvt snd_conv)
-  apply (clarsimp, rule_tac x = "s" in exI, simp)
-  apply (subgoal_tac "agrees (fvB guard) (fst \<sigma>) s")
-   apply (simp add: bexp_agrees rered.red_BasicEvt)
-  using fvREv_def by auto
-
-lemma reaborts_agrees[rule_format]:
-  "reaborts re \<sigma> \<Longrightarrow> \<forall>s'. agrees (fvREv re) (fst \<sigma>) s' \<longrightarrow> snd \<sigma> = h' \<longrightarrow> reaborts re (s', h')"
-  apply (induct re, simp add: fvREv_def reaborts_equiv)
-  by (simp add: eaborts_agrees)
-
 subsection \<open>functions for event system \<close>
 
 subsubsection \<open>locks that a  event system is currently holding \<close>
@@ -360,30 +194,31 @@ subsubsection \<open>locks that a  event system is currently holding \<close>
 primrec
   eslocked :: "esys \<Rightarrow> rname set"
   where
-  "eslocked (EvtSeq re esys) = relocked re"
+  "eslocked (EvtSeq e esys) = elocked e"
 | "eslocked (EvtSys _) = {}"
 
 primrec
   esllocked :: "esys \<Rightarrow> rname list"
   where
-  "esllocked (EvtSeq re esys) = rellocked re"
+  "esllocked (EvtSeq e esys) = ellocked e"
 | "esllocked (EvtSys S) = []"
 
+
 lemma eslocked_eq: "eslocked es = set (esllocked es)"
-  by (induct es, simp_all add: elocked_eq rellocked_def relocked_def)
+  by (metis elocked_eq empty_set esllocked.simps(1) esllocked.simps(2) eslocked.simps(1) eslocked.simps(2) esys.exhaust)
 
 subsubsection \<open>memory accesses and memory writes a event system performs in one step \<close>
 
 primrec
   esaccesses :: "esys \<Rightarrow> stack \<Rightarrow> nat set"
   where
-  "esaccesses (EvtSeq re esys) s = reaccesses re s"
+  "esaccesses (EvtSeq e esys) s = eaccesses e s"
 | "esaccesses (EvtSys S) s = {}"
 
 primrec
   eswrite :: "esys \<Rightarrow> stack \<Rightarrow> nat set"
   where
-  "eswrite (EvtSeq re esys) s = rewrite re s"
+  "eswrite (EvtSeq e esys) s = ewrite e s"
 | "eswrite (EvtSys S) s = {}"
 
 subsubsection \<open>A event system aborts in a given state\<close>
@@ -391,189 +226,76 @@ subsubsection \<open>A event system aborts in a given state\<close>
 inductive 
   esaborts :: "esys \<Rightarrow> state \<Rightarrow> bool"
   where
-  aborts_EvtSeq: "reaborts re \<sigma> \<Longrightarrow> esaborts (EvtSeq re esys) \<sigma>"
-| aborts_EvtSys: "re \<in> es  \<Longrightarrow> reaborts re \<sigma> \<Longrightarrow>  esaborts (EvtSys es) \<sigma>"
+  aborts_EvtSeq: "eaborts e \<sigma> \<Longrightarrow> esaborts (EvtSeq e esys) \<sigma>"
+| aborts_EvtSys: "e \<in> es  \<Longrightarrow> eaborts e \<sigma> \<Longrightarrow>  esaborts (EvtSys es) \<sigma>"
 
 subsubsection \<open>free variable of event system\<close>
 
 primrec
   fvEsv :: "esys \<Rightarrow> var set"
   where
-  "fvEsv (EvtSeq re esys) = (fvREv re) \<union> (fvEsv) esys"
-| "fvEsv (EvtSys es) = {x. \<exists>re \<in> es.  x \<in> (fvREv re)}"
+  "fvEsv (EvtSeq e esys) = (fvEv e) \<union> (fvEsv) esys"
+| "fvEsv (EvtSys es) = {x. \<exists>e \<in> es.  x \<in> (fvEv e)}"
 
 subsubsection \<open>all variables may be updated by a event system\<close>
 
 primrec
   wrEsv :: "esys \<Rightarrow> var set"
   where
-  "wrEsv (EvtSeq re esys) = (wrREv re) \<union> (wrEsv esys)"
-| "wrEsv (EvtSys es) = {x. \<exists>re \<in> es. x \<in> (wrREv re)}"
+  "wrEsv (EvtSeq e esys) = (wrEv e) \<union> (wrEsv esys)"
+| "wrEsv (EvtSys es) = {x. \<exists>e \<in> es. x \<in> (wrEv e)}"
                    
 subsubsection \<open>Basic properties about event system semantics\<close>
 
-lemma fvEsv_property : "re \<in> es \<Longrightarrow> fvEsv (EvtSeq re (EvtSys es)) = fvEsv (EvtSys es)"
+lemma fvEsv_property : "e \<in> es \<Longrightarrow> fvEsv (EvtSeq e (EvtSys es)) = fvEsv (EvtSys es)"
   by auto
 
-lemma wrEsv_property : "re \<in> es \<Longrightarrow> wrEsv (EvtSeq re (EvtSys es)) = wrEsv (EvtSys es)"
+lemma wrEsv_property : "e \<in> es \<Longrightarrow> wrEsv (EvtSeq e (EvtSys es)) = wrEsv (EvtSys es)"
   by auto
 
 lemma eswrites_accesses : "eswrite es s \<subseteq> esaccesses es s"
-  by (induct es arbitrary: s, simp_all add : rewrites_accesses)
+  by (induct es arbitrary: s, simp_all add : ewrites_accesses)
 
 lemma esred_properties :
 "(esys, \<sigma>, x) -es-actk\<rightarrow> (esys', \<sigma>', x') \<Longrightarrow> fvEsv esys' \<subseteq> fvEsv esys 
                          \<and> wrEsv esys' \<subseteq> wrEsv esys \<and> agrees (- wrEsv esys) (fst \<sigma>) (fst \<sigma>')"
   apply (erule esred.cases, simp_all)
-    apply (simp add: le_supI1 rered_properties agrees_def)
-    apply (metis (mono_tags, lifting) IntD1 agrees_def rered_properties)
-  apply (meson Int_lower1 agreesC agrees_search(2) rered_properties)
+    apply (simp add: le_supI1 ered_properties agrees_def)
+    apply (metis (mono_tags, lifting) IntD1 agrees_def ered_properties)
+  apply (meson Int_lower1 agreesC agrees_search(2) ered_properties)
   apply (rule conjI, clarsimp)
-   apply (meson contra_subsetD rered_properties)
+   apply (meson contra_subsetD ered_properties)
   apply (rule conjI, clarsimp)
-   apply (meson contra_subsetD rered_properties, clarsimp)
-  using rered_properties by fastforce
+  using ered_properties apply blast
+  using ered_properties by fastforce
 
 lemma esaccesses_agrees: 
 "agrees (fvEsv esys) s s' \<Longrightarrow> esaccesses esys s = esaccesses esys s'"
   apply (induct esys arbitrary: s s', simp_all add: exp_agrees, clarsimp)
-  by (simp add: reaccesses_agrees)
+  by (simp add: eaccesses_agrees)
 
 lemma eswrites_agrees: 
 "agrees (fvEsv esys) s s' \<Longrightarrow> eswrite esys s = eswrite esys s'"
   apply (induct esys arbitrary: s s', simp_all add: exp_agrees, clarsimp)
-  by (simp add: rewrites_agrees)
+  by (simp add: ewrites_agrees)
 
 lemma esred_agrees[rule_format] : 
 "(esys, \<sigma>, x) -es-actk\<rightarrow> (esys', \<sigma>', x') \<Longrightarrow> \<forall>X s. agrees X (fst \<sigma>) s \<longrightarrow> snd \<sigma> = h \<longrightarrow> fvEsv esys \<subseteq> X \<longrightarrow>
    (\<exists>s' h'. (esys, (s, h), x) -es-actk\<rightarrow> (esys', (s', h'), x') \<and> agrees X (fst \<sigma>') s' \<and> snd \<sigma>' = h')"
   apply (erule esred.cases, simp_all, clarsimp)
-    apply (drule_tac X = "X" and s = "s" in rered_agrees, simp_all)
+    apply (drule_tac X = "X" and s = "s" in ered_agrees, simp_all)
     apply (clarsimp, rule_tac x = "s'" in exI, simp add: esred.red_EvtSeq1)
-  apply (meson esred.red_EvtSeq2 rered_agrees snd_conv)
-  apply (clarsimp, drule rered_agrees, simp_all)
+  apply (meson esred.red_EvtSeq2 ered_agrees snd_conv)
+  apply (clarsimp, drule ered_agrees, simp_all)
    apply blast
   using esred.red_EvtSet by blast
 
 lemma esaborts_agrees[rule_format] :
 "esaborts esys \<sigma> \<Longrightarrow> \<forall>s'. agrees (fvEsv esys) (fst \<sigma>) s' \<longrightarrow> snd \<sigma> = h' \<longrightarrow> esaborts esys (s', h')"
   apply (erule esaborts.induct, simp_all)
-   apply (auto simp add: rewrites_agrees reaccesses_agrees exp_agrees, auto simp add: agrees_def)
-   apply (simp add: aborts_EvtSeq agrees_def reaborts_agrees)
-  apply (subgoal_tac "reaborts (a, b) (s', h')", simp add: aborts_EvtSys)
-  by (metis (mono_tags, lifting) agrees_def fst_conv reaborts_agrees snd_conv)
-
-
-
-subsection \<open>functions for resource event system \<close>
-
-subsubsection \<open>locks that a resource event system is currently holding \<close>
-
-definition 
-  reslocked :: "resys \<Rightarrow> rname set"
-  where
-  "reslocked res = eslocked (snd res) - set (fst res)"
-
-definition 
-  resllocked :: "resys \<Rightarrow> rname list"
-  where
-  "resllocked res = list_minus (esllocked (snd res)) (fst res)"
-
-lemma reslocked_eq: "reslocked res = set (resllocked res)"
-  by (simp add: eslocked_eq resllocked_def reslocked_def)
-
-subsubsection \<open>memory accesses and memory writes a resouce event system performs in one step \<close>
-
-definition
-  resaccesses :: "resys \<Rightarrow> stack \<Rightarrow> nat set"
-  where
-  "resaccesses res s = esaccesses (snd res) s"
-
-definition 
-  reswrite :: "resys \<Rightarrow> stack \<Rightarrow> nat set"
-  where
-  "reswrite res s = eswrite (snd res) s"
-
-subsubsection \<open>A resource event system aborts in a given state\<close>
-
-inductive 
-  resaborts :: "resys \<Rightarrow> state \<Rightarrow> bool"
-  where
-  aborts_EvtSeq: " reaborts re \<sigma> \<Longrightarrow> resaborts (rs, (EvtSeq re res)) \<sigma>"
-| aborts_EvtSys: " re \<in> es \<Longrightarrow> reaborts re \<sigma> \<Longrightarrow> resaborts (rs, (EvtSys es)) \<sigma>"
-
-lemma resaborts_equiv : "resaborts res \<sigma> = esaborts (snd res) \<sigma>"
-proof
-  assume "resaborts res \<sigma>"
-  then show "esaborts (snd res) \<sigma>"
-    by (metis esaborts.simps resaborts.cases sndI)
-next
-  assume "esaborts (snd res) \<sigma>"
-  then show "resaborts res \<sigma>"
-    by (metis esaborts.cases prod.collapse resaborts.simps)
-qed
-
-subsubsection \<open>free variable of resource event system\<close>
-
-definition
-  fvREsv :: "resys \<Rightarrow> var set"
-  where
-  "fvREsv resys = fvEsv (snd resys)"
-
-subsubsection \<open>all variables may be updated by a resource event system\<close>
-
-definition
-  wrREsv :: "resys \<Rightarrow> var set"
-  where
-  "wrREsv resys = wrEsv (snd resys)"
-                   
-subsubsection \<open>Basic properties about resource event system semantics\<close>
-
-lemma reswrites_accesses : "reswrite res s \<subseteq> resaccesses res s"
-  by (simp add: reswrite_def resaccesses_def eswrites_accesses)
-
-lemma resred_properties :
-"(resys, \<sigma>, x) -res-actk\<rightarrow> (resys', \<sigma>', x') \<Longrightarrow> fvREsv resys' \<subseteq> fvREsv resys 
-                         \<and> wrREsv resys' \<subseteq> wrREsv resys \<and> agrees (- wrREsv resys) (fst \<sigma>) (fst \<sigma>')"
-  apply (erule resred.cases, simp_all add: fvREsv_def wrREsv_def)
-    apply (metis agrees_search(1) agrees_simps(4) le_supI1 rered_properties sup_inf_absorb)
-   apply (simp add: wrREv_def agrees_refl)
-  apply (metis boolean_algebra.de_Morgan_disj esred.red_EvtSeq2 esred_properties wrEsv.simps(1) wrREv_def)
-  apply (rule conjI, clarsimp)
-  using fvREv_def rered_properties 
-  apply (metis snd_conv subsetD)
-  apply (rule conjI, clarsimp)
-  using rered_properties  wrREv_def 
-  apply (metis snd_conv subsetD)
-  using mem_Collect_eq rered_properties snd_conv wrREv_def 
-  by (simp add: agrees_def)
-
-lemma resaccesses_agrees: 
-"agrees (fvREsv resys) s s' \<Longrightarrow> resaccesses resys s = resaccesses resys s'"
-  apply (induct resys arbitrary: s s', simp add: fvREsv_def resaccesses_def)
-  by (simp add: esaccesses_agrees)
-
-lemma reswrites_agrees: 
-"agrees (fvREsv resys) s s' \<Longrightarrow> reswrite resys s = reswrite resys s'"
-  apply (induct resys arbitrary: s s', simp_all add: fvREsv_def reswrite_def)
-  by (simp add: eswrites_agrees)
-
-lemma resred_agrees[rule_format] : 
-"(resys, \<sigma>, x) -res-actk\<rightarrow> (resys', \<sigma>', x') \<Longrightarrow> \<forall>X s. agrees X (fst \<sigma>) s \<longrightarrow> snd \<sigma> = h \<longrightarrow> fvREsv resys \<subseteq> X \<longrightarrow>
-   (\<exists>s' h'. (resys, (s, h), x) -res-actk\<rightarrow> (resys', (s', h'), x') \<and> agrees X (fst \<sigma>') s' \<and> snd \<sigma>' = h')"
-  apply (erule resred.cases, simp_all add: fvREsv_def wrREsv_def, clarsimp)
-  apply (drule_tac X = "X" and s = "s" in rered_agrees, simp_all)
-    apply (clarsimp, rule_tac x = "s'" in exI, simp add: resred.red_EvtSeq1)
-  apply (meson rered_agrees resred.red_EvtSeq2 snd_conv)
-  apply (clarsimp, drule rered_agrees, simp_all add: fvREv_def)
-  using mem_Collect_eq subset_iff apply fastforce
-  using resred.red_EvtSet by blast
-
-lemma resaborts_agrees[rule_format] :
-"resaborts resys \<sigma> \<Longrightarrow> \<forall>s'. agrees (fvREsv resys) (fst \<sigma>) s' 
-                      \<longrightarrow> snd \<sigma> = h' \<longrightarrow> resaborts resys (s', h')"
-  apply (simp add: resaborts_equiv fvREsv_def)
-  by (simp add: esaborts_agrees)
+   apply (auto simp add: ewrites_agrees eaccesses_agrees exp_agrees, auto simp add: agrees_def)
+   apply (simp add: aborts_EvtSeq agrees_def eaborts_agrees)
+  by (metis (mono_tags, lifting) agrees_def eaborts_agrees esaborts.simps prod.sel(1) prod.sel(2))
 
 subsection \<open>functions for parallel event system \<close>
 
@@ -582,7 +304,7 @@ subsubsection \<open>locks that a parallel system is currently holding \<close>
 definition
   pesllocked :: "paresys \<Rightarrow> rname list"
   where
-  "pesllocked pes = List.maps resllocked pes"
+  "pesllocked pes = List.maps esllocked pes"
 
 definition
   peslocked :: "paresys \<Rightarrow> rname set"
@@ -592,17 +314,17 @@ definition
 lemma empty_peslock : "peslocked [] = {}"
   by (simp add: maps_simps(2) pesllocked_def peslocked_def)
 
-lemma pesllocked_induct : "pesllocked (res # pes) = resllocked res @ pesllocked pes"
+lemma pesllocked_induct : "pesllocked (es # pes) = esllocked es @ pesllocked pes"
   by (simp add: maps_simps(1) pesllocked_def)
 
-lemma peslock_notin : "r \<notin> peslocked pes \<Longrightarrow> \<forall>k < length pes. r \<notin> reslocked (pes ! k)"
-  apply (simp add: peslocked_def pesllocked_def reslocked_eq)
+lemma peslock_notin : "r \<notin> peslocked pes \<Longrightarrow> \<forall>k < length pes. r \<notin> eslocked (pes ! k)"
+  apply (simp add: peslocked_def pesllocked_def eslocked_eq)
   apply (induct pes, simp, clarsimp)
   apply (case_tac k, simp add: maps_simps(1))
   by (simp add: maps_simps(1))
 
-lemma induct_peslock : "peslocked (x # xs) = (reslocked x) \<union> peslocked (xs)"
-  by (simp add: maps_simps(1) pesllocked_def peslocked_def reslocked_eq)
+lemma induct_peslock : "peslocked (x # xs) = (eslocked x) \<union> peslocked (xs)"
+  by (simp add: maps_simps(1) pesllocked_def peslocked_def eslocked_eq)
 
 lemma peslocked_eq : "set (pesllocked pes) = peslocked pes"
   by (simp add: peslocked_def)
@@ -612,17 +334,17 @@ lemma maps_append : "List.maps f (l1 @ l2) = List.maps f l1 @ List.maps f l2"
   by (simp add: List.append.append_Cons maps_simps)
 
 lemma peslocked_split : "k < length pes \<Longrightarrow> pesllocked pes = 
-       pesllocked (take k pes) @ resllocked (pes ! k) @ pesllocked (drop (Suc k) pes)"
+       pesllocked (take k pes) @ esllocked (pes ! k) @ pesllocked (drop (Suc k) pes)"
 proof-
   assume a0: "k < length pes"
   then have " pes = take k pes @ (pes ! k) # drop (Suc k) pes"
     by (simp add: id_take_nth_drop)
   then have "pesllocked pes = pesllocked (take k pes @ (pes ! k) # drop (Suc k) pes)"
     by simp
-  then have "pesllocked pes = List.maps resllocked (take k pes @ (pes ! k) # drop (Suc k) pes)"
+  then have "pesllocked pes = List.maps esllocked (take k pes @ (pes ! k) # drop (Suc k) pes)"
     by (simp add: pesllocked_def)
-  then have "pesllocked pes = List.maps resllocked (take k pes) 
-           @ resllocked (pes ! k) @ List.maps resllocked (drop (Suc k) pes)"
+  then have "pesllocked pes = List.maps esllocked (take k pes) 
+           @ esllocked (pes ! k) @ List.maps esllocked (drop (Suc k) pes)"
     by (simp add: maps_append maps_simps(1))
   then show ?thesis
     by (simp add: pesllocked_def)
@@ -631,18 +353,18 @@ qed
 inductive
   pesred :: "pesconf \<Rightarrow> actk \<Rightarrow> pesconf \<Rightarrow> bool" ("_ -pes-_\<rightarrow> _" [81,81,81] 80)
   where
-  red_Par : "\<lbrakk>k < length pes;  pes ! k = res ; (res, \<sigma>, x) -res-(a\<sharp>k)\<rightarrow> (res', \<sigma>', x');
-             \<forall>k'. k' < length pes \<and> k \<noteq> k' \<longrightarrow> disjoint (reslocked res') (reslocked (pes ! k'))\<rbrakk> 
-             \<Longrightarrow> (pes, \<sigma>, x) -pes-a\<sharp>k\<rightarrow> ((pes[k := res']), \<sigma>', x')"
+  red_Par : "\<lbrakk>k < length pes;  pes ! k = es ; (es, \<sigma>, x) -es-(a\<sharp>k)\<rightarrow> (es', \<sigma>', x');
+             \<forall>k'. k' < length pes \<and> k \<noteq> k' \<longrightarrow> disjoint (eslocked es') (eslocked (pes ! k'))\<rbrakk> 
+             \<Longrightarrow> (pes, \<sigma>, x) -pes-a\<sharp>k\<rightarrow> ((pes[k := es']), \<sigma>', x')"
 
 subsubsection \<open>A parallel system aborts in a given state\<close>
 
 inductive
   pesaborts :: "paresys \<Rightarrow> state \<Rightarrow> bool"
   where
-  aborts_Par : " \<exists>k. k < length  pes \<and> resaborts (pes ! k) \<sigma> \<Longrightarrow> pesaborts pes \<sigma>"
-| aborts_Race : "\<exists>k1 k2. k1 < length pes \<and> k2 < length pes \<and> k1 \<noteq> k2  \<and> \<not> disjoint (resaccesses (pes ! k1) (fst \<sigma>)) 
-                         (reswrite (pes ! k2) (fst \<sigma>)) \<Longrightarrow> pesaborts pes \<sigma>"
+  aborts_Par : " \<exists>k. k < length pes \<and> esaborts (pes ! k) \<sigma> \<Longrightarrow> pesaborts pes \<sigma>"
+| aborts_Race : "\<exists>k1 k2. k1 < length pes \<and> k2 < length pes \<and> k1 \<noteq> k2  \<and> \<not> disjoint (esaccesses (pes ! k1) (fst \<sigma>)) 
+                 (eswrite (pes ! k2) (fst \<sigma>)) \<Longrightarrow> pesaborts pes \<sigma>"
 
 subsubsection \<open>memory accesses and memory writes a parallel event system performs in one step \<close>
 
@@ -650,13 +372,13 @@ primrec
   pesaccesses :: "paresys \<Rightarrow> stack \<Rightarrow> nat set"
   where
   "pesaccesses [] s = {}"
-| "pesaccesses (res # pes) s = (resaccesses res s) \<union> (pesaccesses pes s)"
+| "pesaccesses (es # pes) s = (esaccesses es s) \<union> (pesaccesses pes s)"
 
 primrec
   peswrite :: "paresys \<Rightarrow> stack \<Rightarrow> nat set"
   where
   "peswrite [] s = {}"
-| "peswrite (res # pes) s = (reswrite res s) \<union> (peswrite pes s)"
+| "peswrite (es # pes) s = (eswrite es s) \<union> (peswrite pes s)"
 
 subsubsection \<open>free variable of parallel event system\<close>
 
@@ -664,7 +386,7 @@ fun
   fvPEsv :: "paresys \<Rightarrow> var set"
   where
   "fvPEsv [] = {}"
-| "fvPEsv (res # pes) = (fvREsv res) \<union> (fvPEsv pes)"
+| "fvPEsv (es # pes) = (fvEsv es) \<union> (fvPEsv pes)"
 
 subsubsection \<open>all variables may be updated by a parallel event system\<close>
 
@@ -672,48 +394,46 @@ fun
   wrPEsv :: "paresys \<Rightarrow> var set"
   where 
   "wrPEsv [] = {}"
-| "wrPEsv (res # pes) = (wrREsv res) \<union> (wrPEsv pes)"
+| "wrPEsv (es # pes) = (wrEsv es) \<union> (wrPEsv pes)"
 
 lemma peswrites_accesses : "peswrite pes s \<subseteq> pesaccesses pes s"
   apply (induct pes, simp, simp)
-  apply (rule conjI, simp add: le_supI1 reswrites_accesses)
+  apply (rule conjI, simp add: le_supI1 eswrites_accesses)
   by (simp add: le_supI2)
 
-lemma K1 : "fvPEsv pes \<subseteq> A \<longleftrightarrow> (\<forall>res \<in> set pes. fvREsv res \<subseteq> A)"
+lemma K1 : "fvPEsv pes \<subseteq> A \<longleftrightarrow> (\<forall>es \<in> set pes. fvEsv es \<subseteq> A)"
   by (induct pes, simp, simp)
 
-lemma K2 : "wrPEsv pes \<subseteq> A \<longleftrightarrow> (\<forall>res \<in> set pes. wrREsv res \<subseteq> A)"
+lemma K2 : "wrPEsv pes \<subseteq> A \<longleftrightarrow> (\<forall>es \<in> set pes. wrEsv es \<subseteq> A)"
   by (induct pes, simp, simp)
 
-lemma fvPEsv_equiv : "fvPEsv pes = {x. \<exists>res \<in> set pes. x \<in> fvREsv res}"
+lemma fvPEsv_equiv : "fvPEsv pes = {x. \<exists>es \<in> set pes. x \<in> fvEsv es}"
   by (induct pes, simp, simp add: Collect_disj_eq)
 
-lemma wrPEsv_equiv : "wrPEsv pes = {x. \<exists>res \<in> set pes. x \<in> wrREsv res}"
+lemma wrPEsv_equiv : "wrPEsv pes = {x. \<exists>es \<in> set pes. x \<in> wrEsv es}"
   by (induct pes, simp, simp add: Collect_disj_eq)
 
 lemma pesred_properties:
   "(pes, \<sigma>, x) -pes-actk\<rightarrow> (pes', \<sigma>', x') \<Longrightarrow> fvPEsv pes' \<subseteq> fvPEsv pes \<and> wrPEsv pes' \<subseteq> wrPEsv pes 
           \<and> agrees (- wrPEsv pes) (fst \<sigma>') (fst \<sigma>)"
   apply (erule pesred.cases, simp_all)
-  apply (simp add: le_supI1 resred_properties agrees_def fvPEsv_equiv wrPEsv_equiv)
+  apply (simp add: le_supI1 esred_properties agrees_def fvPEsv_equiv wrPEsv_equiv)
   apply (rule conjI, clarsimp)
    apply (metis (no_types, lifting) insertE nth_mem 
-            resred_properties set_update_subset_insert subset_iff)
+          esred_properties set_update_subset_insert subset_iff)
   apply (rule conjI, clarsimp)
-   apply (metis (no_types, lifting) insertE nth_mem resred_properties 
-        set_update_subset_insert subset_eq subset_iff, clarsimp)
-  by (metis (mono_tags, lifting) ComplI agrees_def fst_conv list_update_id 
-            resred_properties set_update_memI)
+   apply (metis (no_types, lifting) insertE nth_mem esred_properties set_update_subset_insert  subset_iff, clarsimp)
+  by (metis (mono_tags, lifting) ComplI agrees_def  list_update_id esred_properties set_update_memI)
 
 lemma pesaccesses_agrees:
   "agrees (fvPEsv pes) s s' \<Longrightarrow> pesaccesses pes s = pesaccesses pes s'"
   apply (induct pes arbitrary: s s', simp_all)
-  using resaccesses_agrees by blast
+  using esaccesses_agrees by blast
 
 lemma peswrites_agrees:
   "agrees (fvPEsv pes) s s' \<Longrightarrow> peswrite pes s = peswrite pes s'"
   apply (induct pes arbitrary: s s', simp_all)
-  using reswrites_agrees by blast
+  using eswrites_agrees by blast
 
 subsection \<open>functions for resource parallel event system \<close>
 
@@ -738,8 +458,8 @@ lemma rpeslocked_eq : "set (rpesllocked rpes) = rpeslocked rpes"
 inductive
   rpesred :: "rpesconf \<Rightarrow> actk \<Rightarrow> rpesconf \<Rightarrow> bool" ("_ -rpes-_\<rightarrow> _" [81,81,81] 80)
   where
-  red_Par: "\<lbrakk>k < length pes;  pes ! k = res ; (res, \<sigma>, x) -res-(a\<sharp>k)\<rightarrow> (res', \<sigma>', x');
-             \<forall>k'. k' < length pes \<and> k \<noteq> k' \<longrightarrow> disjoint (reslocked res') (reslocked (pes ! k'))\<rbrakk> 
+  red_Par: "\<lbrakk>k < length pes;  pes ! k = res ; (res, \<sigma>, x) -es-(a\<sharp>k)\<rightarrow> (res', \<sigma>', x');
+             \<forall>k'. k' < length pes \<and> k \<noteq> k' \<longrightarrow> disjoint (eslocked res') (eslocked (pes ! k'))\<rbrakk> 
           \<Longrightarrow> ((r, pes), \<sigma>, x) -rpes-a\<sharp>k\<rightarrow> ((r, pes[k := res']), \<sigma>', x')"
 
 lemma rpes_invres : "(rpes, \<sigma>, x)-rpes-actk\<rightarrow> (rpes', \<sigma>', x') \<Longrightarrow> fst rpes = fst rpes'"
@@ -759,11 +479,11 @@ subsubsection \<open>A resource parallel system aborts in a given state\<close>
 inductive
   rpesaborts :: "rparesys \<Rightarrow> state \<Rightarrow> bool"
   where
-  aborts_Par : " \<exists>k. k < length pes \<and> resaborts  (pes ! k) \<sigma> 
+  aborts_Par : " \<exists>k. k < length pes \<and> esaborts  (pes ! k) \<sigma> 
                  \<Longrightarrow> rpesaborts (r, pes) \<sigma>"
 | aborts_Race : "\<exists>k1 k2. k1 < length pes \<and> k2 < length pes \<and> k1 \<noteq> k2  \<and> 
-                  \<not> disjoint (resaccesses (pes ! k1) (fst \<sigma>)) 
-                         (reswrite (pes ! k2) (fst \<sigma>)) \<Longrightarrow> rpesaborts (r, pes) \<sigma>"
+                  \<not> disjoint (esaccesses (pes ! k1) (fst \<sigma>)) 
+                         (eswrite (pes ! k2) (fst \<sigma>)) \<Longrightarrow> rpesaborts (r, pes) \<sigma>"
 
 lemma rpesaborts_equiv : "rpesaborts (r, pes) \<sigma> = pesaborts pes \<sigma>"
 proof
@@ -771,7 +491,7 @@ proof
   then show "pesaborts pes \<sigma>"
     apply (rule rpesaborts.cases, simp_all)
     apply (simp add: pesaborts.aborts_Par)
-    by (simp add: pesaborts.aborts_Race resaccesses_def reswrite_def)
+    by (simp add: pesaborts.aborts_Race esaccesses_def eswrite_def)
 next
   assume "pesaborts pes \<sigma>"
   then show "rpesaborts (r, pes) \<sigma>"
