ReCore_IFS.thy
@@ -1,0 +1,8 @@
+theory ReCore_IFS
+  imports SecurityModel Lang
+begin
+
+record  action = 
+        actk :: " actk"
+        eventof :: "('l,'k,'s, 'prog) event"
+        domain ::  "'d"
